src/tls/CommonDH.fst
@@ -1,32 +1,65 @@
 (*--build-config
 options:--use_hints --fstar_home ../../../FStar --include ../../../FStar/ucontrib/Platform/fst/ --include ../../../FStar/ucontrib/CoreCrypto/fst/ --include ../../../FStar/examples/low-level/crypto/real --include ../../../FStar/examples/low-level/crypto/spartan --include ../../../FStar/examples/low-level/LowCProvider/fst --include ../../../FStar/examples/low-level/crypto --include ../../libs/ffi --include ../../../FStar/ulib/hyperstack --include ideal-flags;
 --*)
+(**
+An abstract interface for Diffie-Hellman operations
+
+When the key extraction stack is idealized (ideal_KEF), this module
+records the honesty of shares using two layers of types: pre_share
+is for syntactically valid shares (used in parsing modules) while
+share is for registered shares (for which is_honest is defined).
+*)
 ﻿module CommonDH
 
+open FStar.HyperStack
 open Platform.Bytes
 open Platform.Error
 open CoreCrypto
 open TLSConstants
 open TLSError
+open FStar.ST
+
+module MR = FStar.Monotonic.RRef
+module MM = MonotoneMap
 
 type group =
   | FFDH of DHGroup.group
   | ECDH of ECGroup.group
 
-type keyshare (g:group) =
+type pre_keyshare (g:group) =
   (match g with
   | FFDH dhg -> DHGroup.keyshare dhg
   | ECDH ecg -> ECGroup.keyshare ecg)
 
-type share (g:group) =
+type pre_share (g:group) =
   (match g with
   | FFDH dhg -> DHGroup.share dhg
   | ECDH ecg -> ECGroup.share ecg)
+
+type id = g:group & s:pre_share g
+type honest (i:id) = bool
+
+(* Global log of honestly generated DH shares *)
+private let dh_region:rgn = new_region tls_tables_region
+private type ideal_log = MM.t dh_region id honest (fun _ -> True)
+private type share_table = (if Flags.ideal_KEF then ideal_log else unit)
+
+abstract let share_log: share_table =
+  (if Flags.ideal_KEF then
+    MM.alloc #dh_region #id #honest #(fun _ -> True)
+  else
+    ())
 
 type secret (g:group) =
   (match g with
   | FFDH dhg -> DHGroup.secret dhg
   | ECDH ecg -> ECGroup.secret ecg)
+
+let namedGroup_of_group (g:group) : Tot (option namedGroup) =
+  match g with
+  | ECDH ec -> Some (SEC ec)
+  | FFDH (DHGroup.Named ng) -> Some (FFDHE ng)
+  | _ -> None
 
 val group_of_namedGroup: namedGroup -> Tot (option group)
 let group_of_namedGroup g =
@@ -35,63 +68,221 @@ let group_of_namedGroup g =
   | FFDHE dhe -> Some (FFDH (DHGroup.Named dhe))
   | _ -> None
 
-val pubshare: #g:group -> keyshare g -> Tot (share g)
-let pubshare #g ks =
+val default_group: group
+let default_group = ECDH (CoreCrypto.ECC_P256)
+
+type registered (i:id) =
+  (if Flags.ideal_KEF then
+    let log : ideal_log = share_log in
+    MR.witnessed (MM.defined log i)
+  else
+    True)
+
+type honest_share (i:id) =
+  (if Flags.ideal_KEF then
+    let log : ideal_log = share_log in
+    MR.witnessed (MM.contains log i true)
+  else False)
+
+type dishonest_share (i:id) =
+  (if Flags.ideal_KEF then
+    let log : ideal_log = share_log in
+    MR.witnessed (MM.contains log i false)
+  else True)
+
+val pre_pubshare: #g:group -> pre_keyshare g -> Tot (pre_share g)
+let pre_pubshare #g ks =
   match g with
   | FFDH dhg -> DHGroup.pubshare #dhg ks
   | ECDH ecg -> ECGroup.pubshare #ecg ks
 
-val default_group: group
-let default_group = ECDH (CoreCrypto.ECC_P256)
+type share (g:group) = s:pre_share g{registered (|g, s|)}
+type keyshare (g:group) = s:pre_keyshare g{registered (|g, pre_pubshare s|)}
 
-val keygen: g:group -> St (keyshare g)
-let keygen = function
-  | FFDH g -> DHGroup.keygen g
-  | ECDH g -> ECGroup.keygen g
+let pubshare (#g:group) (s:keyshare g) : Tot (share g) =
+  let gx = pre_pubshare s in
+  cut(registered (|g, gx |)); gx
 
-val dh_responder: #g:group -> share g -> St (keyshare g * secret g)
-let dh_responder #g gx = match g with
-  | FFDH g -> DHGroup.dh_responder #g gx
-  | ECDH g -> ECGroup.dh_responder #g gx
+let is_honest (i:id) : ST bool
+  (requires (fun h -> registered i))
+  (ensures (fun h0 b h1 ->
+    modifies_none h0 h1 /\
+    (if Flags.ideal_KEF then
+      let log : ideal_log = share_log in
+      MM.contains log i b h1 /\
+      (b ==> honest_share i) /\
+      (not b ==> dishonest_share i)
+    else b == false)))
+  =
+  if Flags.ideal_KEF then
+   begin
+    let log : ideal_log = share_log in
+    let h = ST.get () in
+    MR.m_recall log;
+    MR.testify (MM.defined log i);
+    cut(Some? (MM.sel (MR.m_sel h log) i));
+    let b = Some?.v (MM.sel (MR.m_read log) i) in
+    cut(MM.contains log i b h);
+    MM.contains_stable log i b;
+    MR.witness log (MM.contains log i b); b
+   end
+  else false
 
-val dh_initiator: #g:group -> keyshare g -> share g -> St (secret g)
+let lemma_honest_or_dishonest (i:id) : ST unit
+  (requires (fun h -> registered i))
+  (ensures (fun h0 _ h1 -> dishonest_share i \/ honest_share i))
+  =
+  if Flags.ideal_KEF then
+   begin
+    let log : ideal_log = share_log in
+    let h = ST.get () in
+    MR.m_recall log;
+    MR.testify (MM.defined log i);
+    cut(Some? (MM.sel (MR.m_sel h log) i));
+    let b = Some?.v (MM.sel (MR.m_read log) i) in
+    match b with
+    | true ->
+      cut(MM.contains log i true h);
+      MM.contains_stable log i true;
+      MR.witness log (MM.contains log i true)
+    | false ->
+      cut(MM.contains log i false h);
+      MM.contains_stable log i false;
+      MR.witness log (MM.contains log i false)
+   end
+  else ()
+
+let lemma_honest_and_dishonest (i:id)
+  : ST unit
+  (requires (fun h0 -> registered i /\ honest_share i /\ dishonest_share i))
+  (ensures (fun h0 _ h1 -> False))
+  =
+  if Flags.ideal_KEF then
+   begin
+    let h = ST.get () in
+    let log : ideal_log = share_log in
+    MR.m_recall log;
+    MR.testify (MM.defined log i);
+    MR.testify (MM.contains log i true);
+    cut(true = Some?.v (MM.sel (MR.m_sel h log) i));
+    MR.testify (MM.contains log i false);
+    cut(false = Some?.v (MM.sel (MR.m_sel h log) i));
+    cut(False)
+   end
+  else ()
+
+// Reified versions of lemma_honest_and_dishonest
+// ADL: I am not able to prove these, waiting for help from Nik
+type absurd_honest (i:id{registered i /\ dishonest_share i}) = honest_share i
+type absurd_dishonest (i:id{registered i /\ honest_share i}) = dishonest_share i
+assume val lemma_honest_and_dishonest_tot: i:id{registered i /\ dishonest_share i} -> absurd_honest i -> Lemma (False)
+assume val lemma_dishonest_and_honest_tot: i:id{registered i /\ honest_share i} -> absurd_dishonest i -> Lemma (False)
+
+let lemma_dishonest_not_honest (i:id)
+  : ST unit
+  (requires (fun h0 -> registered i /\ dishonest_share i))
+  (ensures (fun h0 _ h1 -> ~(honest_share i)))
+  =
+  if Flags.ideal_KEF then
+   begin
+    let j: i:id{registered i /\ dishonest_share i} = i in
+    FStar.Classical.impl_intro (lemma_honest_and_dishonest_tot j);
+    cut(honest_share i ==> False)
+   end
+  else ()
+
+let lemma_honest_not_dishonest (i:id)
+  : ST unit
+  (requires (fun h0 -> registered i /\ honest_share i))
+  (ensures (fun h0 _ h1 -> ~(dishonest_share i)))
+  =
+  if Flags.ideal_KEF then
+   begin
+    let j: i:id{registered i /\ honest_share i} = i in
+    FStar.Classical.impl_intro (lemma_dishonest_and_honest_tot j);
+    cut(dishonest_share i ==> False)
+   end
+  else ()
+
+#set-options "--z3rlimit 100"
+val keygen: g:group -> ST (keyshare g)
+  (requires (fun h0 -> True))
+  (ensures (fun h0 s h1 ->
+    (if Flags.ideal_KEF then
+      modifies_one dh_region h0 h1 /\
+      honest_share (|g, pubshare s|)
+     else
+      modifies_none h0 h1)))
+let rec keygen g =
+  let gx : pre_keyshare g = match g with
+    | FFDH g -> DHGroup.keygen g
+    | ECDH g -> ECGroup.keygen g
+    in
+  let gx : keyshare g =
+   if Flags.ideal_KEF then
+    begin
+     let log : ideal_log = share_log in
+     let i : id = (| g, pre_pubshare gx |) in
+     MR.m_recall log;
+     match MM.lookup log i with
+     | None ->
+       MM.extend log i true;
+       cut(registered i); cut(honest_share i);
+       let gx : keyshare g = gx in gx
+     | Some _ -> // Bad luck, we generated the same share twice
+       keygen g
+    end
+   else gx in
+  gx
+
+val dh_initiator: #g:group -> keyshare g -> share g -> ST (secret g)
+  (requires (fun h0 -> True))
+  (ensures (fun h0 _ h1 -> modifies_none h0 h1))
 let dh_initiator #g gx gy =
   match g with
   | FFDH g -> DHGroup.dh_initiator #g gx gy
   | ECDH g -> ECGroup.dh_initiator #g gx gy
 
-// Serialize in KeyExchange message format
-val serialize: #g:group -> share g -> Tot bytes
-let serialize #g s =
-  match g with
-  | FFDH g -> DHGroup.serialize #g s
-  | ECDH g -> ECGroup.serialize #g s
+val dh_responder: #g:group -> share g -> ST (keyshare g * secret g)
+  (requires (fun h0 -> True))
+  (ensures (fun h0 (ks,s) h1 ->
+    (if Flags.ideal_KEF then
+      modifies_one dh_region h0 h1 /\
+      honest_share (|g, pubshare ks|)
+     else
+      modifies_none h0 h1)))
+let dh_responder #g gx =
+  let gy = keygen g in
+  let gxy = dh_initiator #g gy gx in
+  (gy, gxy)
 
-val parse_partial: bool -> bytes -> Tot (result ((g:group & share g) * bytes))
-let parse_partial ec p =
-  if ec then
-    begin
-    match ECGroup.parse_partial p with
-    | Correct((|g , s|), rem) -> Correct ((| ECDH g, s |), rem)
-    | Error z -> Error z
-    end
-  else
-    begin
-    match DHGroup.parse_partial p with
-    | Correct((|g, s|), rem) -> Correct ((| FFDH g, s |), rem)
-    | Error z -> Error z
-    end
+#set-options "--z3rlimit 100"
+let register (#g:group) (gx:pre_share g) : ST (share g)
+(requires (fun h0 -> True))
+(ensures (fun h0 s h1 ->
+  (if Flags.ideal_KEF then
+    modifies_one dh_region h0 h1
+   else
+    modifies_none h0 h1)))
+  =
+  if Flags.ideal_KEF then
+   begin
+    let log : ideal_log = share_log in
+    let i : id = (| g, gx |) in
+    MR.m_recall log;
+    match MM.lookup log i with
+    | None ->
+      MM.extend log i false;
+      cut(registered i);
+      cut(dishonest_share i);
+      gx
+    | Some b ->
+      cut(MR.witnessed (MM.defined log i));
+      gx
+   end
+  else gx
 
-// Serialize for keyShare extension
-val serialize_raw: #g:group -> share g -> Tot bytes
-let serialize_raw #g s =
-  match g with
-  | FFDH g ->
-    let dhp = DHGroup.params_of_group g in
-    DHGroup.serialize_public #g s (length dhp.dh_p)
-  | ECDH g -> ECGroup.serialize_point #g s
-
-val parse: g:group -> bytes -> Tot (option (share g))
+val parse: g:group -> bytes -> Tot (option (pre_share g))
 let parse g x =
   match g with
   | ECDH g -> ECGroup.parse_point g x
@@ -99,6 +290,39 @@ let parse g x =
     let dhp = DHGroup.params_of_group g in
     if length x = length dhp.dh_p then Some x
     else None
+
+val parse_partial: bool -> bytes -> Tot (result ((g:group & pre_share g) * bytes))
+let parse_partial ec p =
+  if ec then
+    begin
+    match ECGroup.parse_partial p with
+    | Correct((|g , s|), rem) ->
+      Correct ((| ECDH g, s |), rem)
+    | Error z -> Error z
+    end
+  else
+    begin
+    match DHGroup.parse_partial p with
+    | Correct((|g, s|), rem) ->
+      Correct ((| FFDH g, s |), rem)
+    | Error z -> Error z
+    end
+
+// Serialize in KeyExchange message format
+val serialize: #g:group -> pre_share g -> Tot bytes
+let serialize #g s =
+  match g with
+  | FFDH g -> DHGroup.serialize #g s
+  | ECDH g -> ECGroup.serialize #g s
+
+// Serialize for keyShare extension
+val serialize_raw: #g:group -> pre_share g -> Tot bytes
+let serialize_raw #g s =
+  match g with
+  | FFDH g ->
+    let dhp = DHGroup.params_of_group g in
+    DHGroup.serialize_public #g s (length dhp.dh_p)
+  | ECDH g -> ECGroup.serialize_point #g s
 
 (*
 val key_params: key -> Tot params
