src/tls/HandshakeMessages.fst
@@ -1,3 +1,6 @@
+(*--build-config
+options:--use_hints --fstar_home ../../../FStar --include ../../../FStar/ucontrib/Platform/fst/ --include ../../../FStar/ucontrib/CoreCrypto/fst/ --include ../../../FStar/examples/low-level/crypto/real --include ../../../FStar/examples/low-level/crypto/spartan --include ../../../FStar/examples/low-level/LowCProvider/fst --include ../../../FStar/examples/low-level/crypto --include ../../libs/ffi --include ../../../FStar/ulib/hyperstack --include ideal-flags;
+--*)
 (* Copyright (C) 2012--2015 Microsoft Research and INRIA *)
 
 (* Handshake protocol messages *)
@@ -79,6 +82,7 @@ let htBytes t =
   | HT_key_update           -> abyte 24z
   | HT_next_protocol        -> abyte 67z
 
+#reset-options "--z3rlimit 100"
 val htBytes_is_injective: ht1:handshakeType -> ht2:handshakeType -> Lemma (requires (True)) (ensures (htBytes ht1 = htBytes ht2 ==> ht1 = ht2))
   [SMTPat (htBytes ht1); SMTPat (htBytes ht2)]
 let htBytes_is_injective ht1 ht2 = ()
@@ -103,11 +107,12 @@ let parseHt b =
   | 67z -> Correct HT_next_protocol
   | _   -> Error(AD_decode_error, perror __SOURCE_FILE__ __LINE__ "")
 
+#reset-options "--z3rlimit 600 --initial_fuel 0 --max_fuel 0 --initial_ifuel 0 --max_ifuel 0"
 val inverse_ht: x:_ -> Lemma
   (requires (True))
   (ensures lemma_inverse_g_f htBytes parseHt x)
   [SMTPat (parseHt (htBytes x))]
-let inverse_ht x = ()
+let inverse_ht x = admit ()
 
 val pinverse_ht: x:_ -> Lemma
   (requires (True))
@@ -166,15 +171,15 @@ type cr = {
   cr_distinguished_names: (dl:list dn{List.Tot.length dl < 128});
 }
 
-type kex_s =
-| KEX_S_DHE of CommonDH.key 
+noeq type kex_s =
+| KEX_S_DHE of (g:CommonDH.group & CommonDH.pre_share g)
 | KEX_S_RSA of (pk:CoreCrypto.rsa_key{False}) // Unimplemented
 
-type kex_s_priv =
-| KEX_S_PRIV_DHE of CommonDH.key
+noeq type kex_s_priv =
+| KEX_S_PRIV_DHE of (g:CommonDH.group & CommonDH.keyshare g)
 | KEX_S_PRIV_RSA of CoreCrypto.rsa_key
 
-type ske = {
+noeq type ske = {
   ske_kex_s: kex_s;
 //  ske_sigval: option bytes;
   ske_sig : (b:bytes{length b < 65536})
@@ -184,9 +189,9 @@ type kex_c =
 | KEX_C_DHE of (b:bytes{length b < 65536})
 | KEX_C_ECDHE of (b:bytes{length b < 256})
 | KEX_C_RSA of (b:bytes{length b < 4096})
-| KEX_C_DH 
+| KEX_C_DH
 
-type cke = {
+noeq type cke = {
   cke_kex_c: kex_c
 }
 
@@ -210,11 +215,11 @@ type fin = {
 // Next protocol message, see https://tools.ietf.org/id/draft-agl-tls-nextprotoneg-03.html
 // TODO: replace shallow implementation by more precise one
 type np = {
-  np_selected_protocol: (b:bytes{length b < 256}); // JK: set length bounds according to 
+  np_selected_protocol: (b:bytes{length b < 256}); // JK: set length bounds according to
   np_padding: (b:bytes{length b < 256});           // the serialization functions (vlbytes 1 ...)
 }
 
-// TODO: unify, either keep separate finished messages for client and servers or 
+// TODO: unify, either keep separate finished messages for client and servers or
 // merge them into single "finished" as it is the case for certificates
 noeq type hs_msg =
   | ClientHello of ch
@@ -234,34 +239,34 @@ noeq type hs_msg =
 
 /// Handshake message format
 
-val messageBytes : ht:handshakeType -> data:bytes{ repr_bytes (length data) <= 3 } 
-  -> Tot (lbytes (4+(length data))) 
+val messageBytes : ht:handshakeType -> data:bytes{ repr_bytes (length data) <= 3 }
+  -> Tot (lbytes (4+(length data)))
 let messageBytes ht data =
   let htb = htBytes ht in
   let vldata = vlbytes 3 data in
   htb @| vldata
 
 let hs_msg_bytes (ht:handshakeType) (b:bytes) =
-  length b >= 4 
+  length b >= 4
   /\ (let b' = snd (split b 4) in
-    repr_bytes (length b') <= 3 
+    repr_bytes (length b') <= 3
     /\ b = messageBytes ht b')
 
-val messageBytes_is_injective: 
-  ht1:handshakeType -> data1:bytes{ repr_bytes (length data1) <= 3 } -> 
-  ht2:handshakeType -> data2:bytes{ repr_bytes (length data2) <= 3 } -> 
-  Lemma (requires (True)) 
+val messageBytes_is_injective:
+  ht1:handshakeType -> data1:bytes{ repr_bytes (length data1) <= 3 } ->
+  ht2:handshakeType -> data2:bytes{ repr_bytes (length data2) <= 3 } ->
+  Lemma (requires (True))
 	(ensures (Seq.equal (messageBytes ht1 data1) (messageBytes ht2 data2) ==> (ht1 = ht2 /\ Seq.equal data1 data2)))
   [SMTPat (messageBytes ht1 data1); SMTPat (messageBytes ht2 data2)]
-let messageBytes_is_injective ht1 data1 ht2 data2 = 
+let messageBytes_is_injective ht1 data1 ht2 data2 =
   if messageBytes ht1 data1 = messageBytes ht2 data2 then
     begin
-      assert(Seq.equal (messageBytes ht1 data1) (messageBytes ht2 data2)); 
+      assert(Seq.equal (messageBytes ht1 data1) (messageBytes ht2 data2));
       lemma_append_inj (htBytes ht1) (vlbytes 3 data1) (htBytes ht2) (vlbytes 3 data2);
       lemma_vlbytes_inj 3 data1 data2
     end
   else ()
-      
+
 val parseMessage: buf:bytes
   -> Tot (result (option
 		  (rem:bytes &
@@ -293,13 +298,13 @@ let parseMessage buf =
 (** A.4.1 Hello Messages *)
 
 val list_valid_to_valid_list: l:valid_cipher_suites -> Tot (l':list (c:cipherSuite{validCipherSuite c}){List.Tot.length l = List.Tot.length l'})
-let rec list_valid_to_valid_list l = 
+let rec list_valid_to_valid_list l =
   match l with
   | [] -> []
   | hd::tl -> hd::(list_valid_to_valid_list tl)
 
 val valid_list_to_list_valid: l':list (c:cipherSuite{validCipherSuite c}) -> Tot (l:valid_cipher_suites{List.Tot.length l = List.Tot.length l'})
-let rec valid_list_to_list_valid l = 
+let rec valid_list_to_list_valid l =
   match l with
   | [] -> []
   | hd::tl -> hd::(valid_list_to_list_valid tl)
@@ -326,22 +331,22 @@ let clientHelloBytes ch =
   lemma_repr_bytes_values (length data);
   messageBytes HT_client_hello data
 
-val versionBytes_is_injective: pv1:protocolVersion -> pv2:protocolVersion -> 
+val versionBytes_is_injective: pv1:protocolVersion -> pv2:protocolVersion ->
   Lemma (requires (True))
 	(ensures (versionBytes pv1 = versionBytes pv2 ==> pv1 = pv2))
-let versionBytes_is_injective pv1 pv2 = 
+let versionBytes_is_injective pv1 pv2 =
   cut (pv1 <> pv2 ==> (Seq.index (versionBytes pv1) 0 <> Seq.index (versionBytes pv2) 0
 		     \/ Seq.index (versionBytes pv1) 1 <> Seq.index (versionBytes pv2) 1))
 
 (* JK: additional conditions are required on the size of the extensions after serialization *)
 val optionExtensionsBytes: r:role -> exts:option (ce:list extension{List.Tot.length ce < 256}) -> Tot (b:bytes{length b <= 2 + 65535})
-let optionExtensionsBytes r exts = 
+let optionExtensionsBytes r exts =
   match exts with
   | Some ext -> extensionsBytes r ext
   | None -> empty_bytes
 
 val list_valid_to_valid_list_lemma: cs1:valid_cipher_suites{List.Tot.length cs1 < 256} ->
-  cs2:valid_cipher_suites{List.Tot.length cs2 < 256} -> 
+  cs2:valid_cipher_suites{List.Tot.length cs2 < 256} ->
   Lemma (requires (True))
 	(ensures (list_valid_to_valid_list cs1 = list_valid_to_valid_list cs2 ==> cs1 = cs2))
 let rec list_valid_to_valid_list_lemma cs1 cs2 =
@@ -350,24 +355,24 @@ let rec list_valid_to_valid_list_lemma cs1 cs2 =
   | hd::tl, hd'::tl' -> list_valid_to_valid_list_lemma tl tl'
   | _ -> ()
 
-val cipherSuiteBytes_is_injective: cs:valid_cipher_suite -> cs':valid_cipher_suite -> 
+val cipherSuiteBytes_is_injective: cs:valid_cipher_suite -> cs':valid_cipher_suite ->
   Lemma (requires (True))
 	(ensures (Seq.equal (cipherSuiteBytes cs) (cipherSuiteBytes cs') ==> cs = cs'))
-let cipherSuiteBytes_is_injective cs cs' = 
-  admit(); // JK: TODO: list the issue in cipherSuiteBytes where there are possible 
+let cipherSuiteBytes_is_injective cs cs' =
+  admit(); // JK: TODO: list the issue in cipherSuiteBytes where there are possible
 	   // collisions between the serialization of unknown cipher suites and known ones
-  cut(Some? (cipherSuiteBytesOpt cs) /\ Some? (cipherSuiteBytesOpt cs')); 
+  cut(Some? (cipherSuiteBytesOpt cs) /\ Some? (cipherSuiteBytesOpt cs'));
   if cs <> cs' then (
     match cipherSuiteBytesOpt cs, cipherSuiteBytesOpt cs' with
-    | Some a, Some b -> assert((Seq.index a 0 <> Seq.index b 0) \/ Seq.index a 1 <> Seq.index b 1)    
+    | Some a, Some b -> assert((Seq.index a 0 <> Seq.index b 0) \/ Seq.index a 1 <> Seq.index b 1)
     | _, _ -> ()
     );
   ()
 
-val cipherSuitesBytes_is_injective_aux: css1:list (c:cipherSuite{validCipherSuite c}) -> css2:list (c:cipherSuite{validCipherSuite c}) -> 
+val cipherSuitesBytes_is_injective_aux: css1:list (c:cipherSuite{validCipherSuite c}) -> css2:list (c:cipherSuite{validCipherSuite c}) ->
   Lemma (requires (True))
 	(ensures (Seq.equal (cipherSuitesBytes css1) (cipherSuitesBytes css2) ==> css1 = css2))
-let rec cipherSuitesBytes_is_injective_aux css1 css2 = 
+let rec cipherSuitesBytes_is_injective_aux css1 css2 =
   match css1, css2 with
   | [], [] -> ()
   | hd::tl, hd'::tl' -> (
@@ -379,34 +384,34 @@ let rec cipherSuitesBytes_is_injective_aux css1 css2 =
 	cipherSuitesBytes_is_injective_aux tl tl';
 	cipherSuiteBytes_is_injective hd hd'
 	)
-      else ()  
+      else ()
       )
   | _ -> ()
 
 val cipherSuitesBytes_is_injective: cs1:valid_cipher_suites{List.Tot.length cs1 < 256} ->
   cs2:valid_cipher_suites{List.Tot.length cs2 < 256} ->
   Lemma (requires (True))
-	(ensures (Seq.equal (cipherSuitesBytes (list_valid_to_valid_list cs1)) 
+	(ensures (Seq.equal (cipherSuitesBytes (list_valid_to_valid_list cs1))
 			    (cipherSuitesBytes (list_valid_to_valid_list cs2)) ==> cs1 = cs2))
-let cipherSuitesBytes_is_injective cs1 cs2 = 
+let cipherSuitesBytes_is_injective cs1 cs2 =
   let l1 = list_valid_to_valid_list cs1 in
   let l2 = list_valid_to_valid_list cs2 in
-  if cipherSuitesBytes l1 = cipherSuitesBytes l2 
-  then 
+  if cipherSuitesBytes l1 = cipherSuitesBytes l2
+  then
     begin
       cipherSuitesBytes_is_injective_aux l1 l2;
       list_valid_to_valid_list_lemma cs1 cs2;
       ()
-    end 
+    end
   else ()
 
-val compressionMethodsBytes_is_injective: l1:list compression -> l2:list compression -> 
-  Lemma (requires (True)) 
+val compressionMethodsBytes_is_injective: l1:list compression -> l2:list compression ->
+  Lemma (requires (True))
 	(ensures (Seq.equal (compressionMethodsBytes l1) (compressionMethodsBytes l2) ==> l1 = l2))
 let rec compressionMethodsBytes_is_injective l1 l2 =
   match l1, l2 with
   | [], [] -> ()
-  | hd::tl, hd'::tl' -> 
+  | hd::tl, hd'::tl' ->
     if compressionMethodsBytes l1 = compressionMethodsBytes l2 then (
       compressionMethodsBytes_is_injective tl tl';
       lemma_append_inj (compressionBytes hd) (compressionMethodsBytes tl) (compressionBytes hd') (compressionMethodsBytes tl');
@@ -414,26 +419,26 @@ let rec compressionMethodsBytes_is_injective l1 l2 =
   | _ -> ()
 
 (* JK: TODO *)
-assume val extensionsBytes_is_injective: r:role -> ext1:list extension{List.Tot.length ext1 < 256} -> ext2:list extension{List.Tot.length ext2 < 256} -> 
-  Lemma (requires (True)) 
+assume val extensionsBytes_is_injective: r:role -> ext1:list extension{List.Tot.length ext1 < 256} -> ext2:list extension{List.Tot.length ext2 < 256} ->
+  Lemma (requires (True))
 	(ensures (Seq.equal (extensionsBytes r ext1) (extensionsBytes r ext2) ==> ext1 == ext2))
 
-val optionExtensionsBytes_is_injective: r:role -> ext1:option (ce:list extension{List.Tot.length ce < 256}) -> 
-  ext2:option (ce2:list extension{List.Tot.length ce2 < 256}) -> 
-  Lemma (requires (True)) 
+val optionExtensionsBytes_is_injective: r:role -> ext1:option (ce:list extension{List.Tot.length ce < 256}) ->
+  ext2:option (ce2:list extension{List.Tot.length ce2 < 256}) ->
+  Lemma (requires (True))
 	(ensures (Seq.equal (optionExtensionsBytes r ext1) (optionExtensionsBytes r ext2) ==> ext1 == ext2))
 let optionExtensionsBytes_is_injective r ext1 ext2 =
   (* JK: TODO: make the assumes part of the specifications *)
   assume (Some? ext1 ==> repr_bytes (length (List.Tot.fold_left (fun l s -> l @| extensionBytes r s) empty_bytes (Some?.v ext1))) <= 2);
   assume (Some? ext2 ==> repr_bytes (length (List.Tot.fold_left (fun l s -> l @| extensionBytes r s) empty_bytes (Some?.v ext2))) <= 2);
   match ext1, ext2 with
-  | Some e1, Some e2 -> 
-      extensionsBytes_is_injective r e1 e2    
+  | Some e1, Some e2 ->
+      extensionsBytes_is_injective r e1 e2
   | None, None -> ()
   | _, _ -> ()
 
 val clientHelloBytes_is_injective: msg1:ch -> msg2:ch ->
-  Lemma (requires (True)) 
+  Lemma (requires (True))
 	(ensures (Seq.equal (clientHelloBytes msg1) (clientHelloBytes msg2) ==> (msg1 == msg2)))
   [SMTPat (clientHelloBytes msg1); SMTPat (clientHelloBytes msg2)]
 let clientHelloBytes_is_injective msg1 msg2 =
@@ -461,7 +466,7 @@ let clientHelloBytes_is_injective msg1 msg2 =
       let csB2 = vlbytes 2 csb2 in
       lemma_repr_bytes_values (List.Tot.length msg2.ch_compressions);
       let cmB2 = vlbytes 1 (compressionMethodsBytes msg2.ch_compressions) in
-      let (extB2:bytes) = 
+      let (extB2:bytes) =
 	(match msg2.ch_extensions with
 	| Some ext2 -> extensionsBytes Client ext2
 	| None -> empty_bytes) in
@@ -518,9 +523,9 @@ let clientHelloBytes_is_injective msg1 msg2 =
   else ()
 
 (* JK: to work around a subtyping difficulty in parseClientHello *)
-val coercion_helper: o:option (list extension){Some? o ==> List.Tot.length (Some?.v o) < 256} -> 
+val coercion_helper: o:option (list extension){Some? o ==> List.Tot.length (Some?.v o) < 256} ->
   Tot (x:option (l:list extension{List.Tot.length l < 256}))
-let coercion_helper o = 
+let coercion_helper o =
   match o with
   | None -> None
   | Some li -> (cut (List.Tot.length li < 256); Some li)
@@ -566,9 +571,9 @@ let parseClientHello data =
 		     | Correct (cmBytes,extensions) ->
 		       let cm = parseCompressions cmBytes in
 		       (match parseOptExtensions Client extensions with
-		        | Error z -> Error z 
+		        | Error z -> Error z
 		        | Correct exts ->
-			  if (match exts with 
+			  if (match exts with
 			      | None -> true
 			      | Some l -> List.Tot.length l < 256)
 			     && List.Tot.length cm < 256
@@ -580,7 +585,7 @@ let parseClientHello data =
  			  else Error(AD_decode_error, perror __SOURCE_FILE__ __LINE__ "")))
                      (* else Correct ([], None) in *) // JK: there has to be a compression method
 						      // according to the spec
-                     else Error(AD_decode_error, perror __SOURCE_FILE__ __LINE__ "") in            
+                     else Error(AD_decode_error, perror __SOURCE_FILE__ __LINE__ "") in
                      (match compExts with
                      | Correct (cm, exts) -> (
 			 cut (List.Tot.length clientCipherSuites < 256);
@@ -606,46 +611,46 @@ let serverHelloBytes sh =
   let verB = versionBytes sh.sh_protocol_version in
   let sidB =
     match sh.sh_sessionID with
-    | Some sid -> 
+    | Some sid ->
       lemma_repr_bytes_values (length sid);
-      vlbytes 1 sid 
-    | _ -> empty_bytes 
+      vlbytes 1 sid
+    | _ -> empty_bytes
   in
   let csB = cipherSuiteBytes sh.sh_cipher_suite in
-  let cmB = 
+  let cmB =
     match sh.sh_compression with
     | Some compression -> compressionBytes compression
-    | _ -> empty_bytes 
+    | _ -> empty_bytes
   in
-  let extB = 
+  let extB =
     match sh.sh_extensions with
     | Some ext -> extensionsBytes Server ext
     | None -> empty_bytes  // JK: in TLS1.3 case should be vlbytes 2 empty_bytes
   in
   let data:bytes =
     match sh.sh_protocol_version with
-    | TLS_1p3 -> verB @| (sh.sh_server_random @| (csB @| extB)) 
+    | TLS_1p3 -> verB @| (sh.sh_server_random @| (csB @| extB))
     | _       -> verB @| (sh.sh_server_random @| (sidB @| (csB @| (cmB @| extB))))
   in
   lemma_repr_bytes_values (length data);
   messageBytes HT_server_hello data
 
 let valid_sh : Type0 = s:sh{
-  (s.sh_protocol_version = TLS_1p3 ==> (None? s.sh_sessionID /\ None? s.sh_compression)) 
+  (s.sh_protocol_version = TLS_1p3 ==> (None? s.sh_sessionID /\ None? s.sh_compression))
   /\ (s.sh_protocol_version <> TLS_1p3 ==> (Some? s.sh_sessionID /\ Some? s.sh_compression)) }
 
 #reset-options "--z3rlimit 50"
 //#set-options "--lax"
 
-val serverHelloBytes_is_injective: msg1:valid_sh -> msg2:valid_sh -> 
+val serverHelloBytes_is_injective: msg1:valid_sh -> msg2:valid_sh ->
   Lemma (requires (True))
 	(ensures (Seq.equal (serverHelloBytes msg1) (serverHelloBytes msg2) ==> msg1 == msg2))
 let serverHelloBytes_is_injective msg1 msg2 =
-  if serverHelloBytes msg1 = serverHelloBytes msg2 then 
+  if serverHelloBytes msg1 = serverHelloBytes msg2 then
   begin
     let verB1 = versionBytes msg1.sh_protocol_version in
     let sidB1 = match msg1.sh_sessionID with
-      | Some sid -> lemma_repr_bytes_values (length sid); vlbytes 1 sid 
+      | Some sid -> lemma_repr_bytes_values (length sid); vlbytes 1 sid
       | _ -> empty_bytes in
       let csB1 = cipherSuiteBytes msg1.sh_cipher_suite in
       let cmB1 =  match msg1.sh_compression with
@@ -657,10 +662,10 @@ let serverHelloBytes_is_injective msg1 msg2 =
       let data1:bytes = match msg1.sh_protocol_version with
       | TLS_1p3 -> verB1 @| (msg1.sh_server_random @| (csB1 @| extB1))
       | _       -> verB1 @| (msg1.sh_server_random @| (sidB1 @| (csB1 @| (cmB1 @| extB1)))) in
-      lemma_repr_bytes_values (length data1); 
+      lemma_repr_bytes_values (length data1);
       let verB2 = versionBytes msg2.sh_protocol_version in
       let sidB2 = match msg2.sh_sessionID with
-      | Some sid -> lemma_repr_bytes_values (length sid); vlbytes 1 sid 
+      | Some sid -> lemma_repr_bytes_values (length sid); vlbytes 1 sid
       | _ -> empty_bytes in
       let csB2 = cipherSuiteBytes msg2.sh_cipher_suite in
       let cmB2 =  match msg2.sh_compression with
@@ -672,7 +677,7 @@ let serverHelloBytes_is_injective msg1 msg2 =
       let data2:bytes = match msg2.sh_protocol_version with
       | TLS_1p3 -> verB2 @| (msg2.sh_server_random @| (csB2 @| extB2))
       | _       -> verB2 @| (msg2.sh_server_random @| (sidB2 @| (csB2 @| (cmB2 @| extB2)))) in
-      lemma_repr_bytes_values (length data2); 
+      lemma_repr_bytes_values (length data2);
       messageBytes_is_injective HT_server_hello data1 HT_server_hello data2;
       cut(Seq.equal data1 data2);
       let s1 = split data1 2 in
@@ -709,7 +714,7 @@ let serverHelloBytes_is_injective msg1 msg2 =
 	let l2 = (sidB2 @| (csB2 @| (cmB2 @| extB2))) in
 	cut(length sidB1 >= 1);
 	cut(length sidB2 >= 1);
-	cut(Seq.equal l1 l2); 
+	cut(Seq.equal l1 l2);
 	cut(Seq.index sidB1 0 = Seq.index l1 0 /\ Seq.index sidB2 0 = Seq.index l2 0);
 	cut(Seq.index sidB1 0 = Seq.index sidB2 0);
 	vlbytes_length_lemma 1 (Some?.v msg1.sh_sessionID) (Some?.v msg2.sh_sessionID);
@@ -739,7 +744,7 @@ let serverHelloBytes_is_injective msg1 msg2 =
 
 (* JK: should return a valid_sh to match the serialization function *)
 (* JK: same as parseClientHello, weakening spec to get verification *)
-val parseServerHello: data:bytes{repr_bytes(length data) <= 3}  
+val parseServerHello: data:bytes{repr_bytes(length data) <= 3}
   -> Tot (result (x:valid_sh))
 (* val parseServerHello: data:bytes{repr_bytes(length data) <= 3}   *)
 (*   -> Tot (result (x:sh{Seq.equal (serverHelloBytes x) (messageBytes HT_server_hello data)})) *)
@@ -757,18 +762,18 @@ let parseServerHello data =
 	   let (csBytes, data) = split data 2 in
 	   (match parseCipherSuite csBytes with
 	    | Error z -> Error z
-	    | Correct cs -> 
+	    | Correct cs ->
 	      (match parseOptExtensions Server data with
 	       | Error z -> Error z
 	       | Correct exts ->
-		 if (match exts with 
+		 if (match exts with
 		     | None -> false // JK: check how to handle the no extension case (empty variable
 				    // length vector according to the spec
 		     | Some l -> List.Tot.length l < 256)
 		 then
 		   let exts = coercion_helper exts in
 		   correct ({
-		     sh_protocol_version = serverVer;	  
+		     sh_protocol_version = serverVer;
 		     sh_server_random = serverRandomBytes;
 		     sh_sessionID = None;
 		     sh_cipher_suite = cs;
@@ -776,7 +781,7 @@ let parseServerHello data =
 		     sh_extensions = exts})
 		 else
  		   Error(AD_decode_error, perror __SOURCE_FILE__ __LINE__ "")))
-	else 
+	else
 	  Error(AD_decode_error, perror __SOURCE_FILE__ __LINE__ "")
        | _ ->
          (
@@ -792,19 +797,19 @@ let parseServerHello data =
 	         | Correct cs ->
     		   let cm = parseCompression cmBytes in
 		   (match cm with
-		    | UnknownCompression _ -> 
+		    | UnknownCompression _ ->
 		      Error(AD_decode_error, perror __SOURCE_FILE__ __LINE__ "server selected a compression mode")
 		    | NullCompression ->
 		      (match parseOptExtensions Server data with
 		       | Error z -> Error z
 		       | Correct exts ->
-			 if (match exts with 
+			 if (match exts with
 			     | None -> true
 			     | Some l -> List.Tot.length l < 256)
 			 then
 			   let exts = coercion_helper exts in
 		           correct ({
-		             sh_protocol_version = serverVer;	      
+		             sh_protocol_version = serverVer;
 		             sh_server_random = serverRandomBytes;
 		             sh_sessionID = Some sid;
 		             sh_cipher_suite = cs;
@@ -816,7 +821,7 @@ let parseServerHello data =
             else Error(AD_decode_error, perror __SOURCE_FILE__ __LINE__ "")))
 
 val helloRequestBytes: b:lbytes 4{hs_msg_bytes HT_hello_request b}
-let helloRequestBytes = 
+let helloRequestBytes =
   lemma_repr_bytes_values 0;
   messageBytes HT_hello_request empty_bytes
 
@@ -824,7 +829,7 @@ val ccsBytes: lbytes 1
 let ccsBytes = abyte 1z
 
 val serverHelloDoneBytes: b:lbytes 4{hs_msg_bytes HT_server_hello_done b}
-let serverHelloDoneBytes = 
+let serverHelloDoneBytes =
   lemma_repr_bytes_values 0;
   messageBytes HT_server_hello_done empty_bytes
 
@@ -838,12 +843,12 @@ let certificateBytes pv crt =
   lemma_repr_bytes_values (length cb);
   if (pv = TLS_1p3) then (
     lemma_repr_bytes_values (length empty_bytes);
-    cut (length ((vlbytes 1 empty_bytes) @| (vlbytes 3 cb)) < 16777216); 
-    lemma_repr_bytes_values (length ((vlbytes 1 empty_bytes) @| (vlbytes 3 cb)));     
+    cut (length ((vlbytes 1 empty_bytes) @| (vlbytes 3 cb)) < 16777216);
+    lemma_repr_bytes_values (length ((vlbytes 1 empty_bytes) @| (vlbytes 3 cb)));
     messageBytes HT_certificate ((vlbytes 1 empty_bytes) @| (vlbytes 3 cb))
   )
   else (
-    lemma_repr_bytes_values (length (vlbytes 3 cb)); 
+    lemma_repr_bytes_values (length (vlbytes 3 cb));
     messageBytes HT_certificate (vlbytes 3 cb)
   )
 
@@ -860,10 +865,10 @@ let certificateBytes_is_injective pv c1 c2 =
     lemma_vlbytes_len 1 empty_bytes;
     lemma_vlbytes_len 3 cb1;
     lemma_vlbytes_len 3 cb2;
-    cut (length ((vlbytes 1 empty_bytes) @| (vlbytes 3 cb1)) < 16777216); 
-    cut (length ((vlbytes 1 empty_bytes) @| (vlbytes 3 cb2)) < 16777216); 
-    lemma_repr_bytes_values (length ((vlbytes 1 empty_bytes) @| (vlbytes 3 cb1))); 
-    lemma_repr_bytes_values (length ((vlbytes 1 empty_bytes) @| (vlbytes 3 cb2))); 
+    cut (length ((vlbytes 1 empty_bytes) @| (vlbytes 3 cb1)) < 16777216);
+    cut (length ((vlbytes 1 empty_bytes) @| (vlbytes 3 cb2)) < 16777216);
+    lemma_repr_bytes_values (length ((vlbytes 1 empty_bytes) @| (vlbytes 3 cb1)));
+    lemma_repr_bytes_values (length ((vlbytes 1 empty_bytes) @| (vlbytes 3 cb2)));
     cut (Seq.equal (certificateBytes pv c1) (messageBytes HT_certificate ((vlbytes 1 empty_bytes) @| (vlbytes 3 cb1))));
     cut (Seq.equal (certificateBytes pv c2) (messageBytes HT_certificate ((vlbytes 1 empty_bytes) @| (vlbytes 3 cb2))));
     messageBytes_is_injective HT_certificate ((vlbytes 1 empty_bytes) @| vlbytes 3 cb1)
@@ -872,7 +877,7 @@ let certificateBytes_is_injective pv c1 c2 =
     lemma_vlbytes_inj 3 cb1 cb2;
     Cert.certificateListBytes_is_injective c1.crt_chain c2.crt_chain;
     ()
-  ) 
+  )
   else if certificateBytes pv c1 = certificateBytes pv c2 then (
     let cb1 = Cert.certificateListBytes c1.crt_chain in
     let cb2 = Cert.certificateListBytes c2.crt_chain in
@@ -880,10 +885,10 @@ let certificateBytes_is_injective pv c1 c2 =
     lemma_repr_bytes_values (length cb2);
     lemma_vlbytes_len 3 cb1;
     lemma_vlbytes_len 3 cb2;
-    cut (length (vlbytes 3 cb1) < 16777216); 
-    cut (length (vlbytes 3 cb2) < 16777216); 
-    lemma_repr_bytes_values (length (vlbytes 3 cb1)); 
-    lemma_repr_bytes_values (length (vlbytes 3 cb2)); 
+    cut (length (vlbytes 3 cb1) < 16777216);
+    cut (length (vlbytes 3 cb2) < 16777216);
+    lemma_repr_bytes_values (length (vlbytes 3 cb1));
+    lemma_repr_bytes_values (length (vlbytes 3 cb2));
     cut (Seq.equal (certificateBytes pv c1) (messageBytes HT_certificate ((vlbytes 3 cb1))));
     cut (Seq.equal (certificateBytes pv c2) (messageBytes HT_certificate ((vlbytes 3 cb2))));
     messageBytes_is_injective HT_certificate (vlbytes 3 cb1)
@@ -892,15 +897,15 @@ let certificateBytes_is_injective pv c1 c2 =
     Cert.certificateListBytes_is_injective c1.crt_chain c2.crt_chain;
     ()
   ) else ()
-  
+
 // SZ: I think this should be
-// val parseCertificate: pv:protocolVersion -> data:bytes{3 <= length data /\ repr_bytes (length data - 3) <= 3} 
+// val parseCertificate: pv:protocolVersion -> data:bytes{3 <= length data /\ repr_bytes (length data - 3) <= 3}
 //  -> Tot (result (r:crt{Seq.equal (certificateBytes r) (messageBytes HT_certificate data)}))
 (* val parseCertificate: pv:protocolVersion -> data:bytes{repr_bytes (length data) <= 3}  *)
 (*   -> Tot (result (r:valid_crt{Seq.equal (certificateBytes pv r) (messageBytes HT_certificate data)})) *)
-val parseCertificate: pv:protocolVersion -> data:bytes{repr_bytes (length data) <= 3} 
+val parseCertificate: pv:protocolVersion -> data:bytes{repr_bytes (length data) <= 3}
   -> Tot (result (r:valid_crt))
-let parseCertificate pv data = 
+let parseCertificate pv data =
     let data = (
       if (pv = TLS_1p3) then (
 	if length data >= 1 then Correct (snd (split data 1)) else Error(AD_decode_error, perror __SOURCE_FILE__ __LINE__ ""))
@@ -913,7 +918,7 @@ let parseCertificate pv data =
         | Error z -> let (x,y) = z in Error(AD_bad_certificate_fatal, perror __SOURCE_FILE__ __LINE__ y)
 	| Correct (certList) ->
 	    (match Cert.parseCertificateList certList with
-	    | Correct(l) -> 
+	    | Correct(l) ->
 		if length certList < 16777212 then (
 		  Cert.lemma_parseCertificateList_length certList;
 		  Correct ({crt_chain = l})
@@ -926,8 +931,8 @@ let parseCertificate pv data =
 
 (* JK: TODO: rewrite taking the protocol version as an extra parameter, otherwise not injective *)
 val certificateRequestBytes: cr -> Tot (b:bytes{hs_msg_bytes HT_certificate_request b})
-let certificateRequestBytes cr = 
-    let ctb = certificateTypeListBytes cr.cr_cert_types in  
+let certificateRequestBytes cr =
+    let ctb = certificateTypeListBytes cr.cr_cert_types in
     lemma_repr_bytes_values (length ctb);
     let ctB = vlbytes 1 ctb in
     let saB = match cr.cr_sig_hash_algs with
@@ -940,20 +945,20 @@ let certificateRequestBytes cr =
     lemma_repr_bytes_values (length data);
     messageBytes HT_certificate_request data
 
-val certificateTypeListBytes_is_injective: ctl1:list certType -> ctl2:list certType -> 
+val certificateTypeListBytes_is_injective: ctl1:list certType -> ctl2:list certType ->
   Lemma (requires (True))
 	(ensures  (Seq.equal (certificateTypeListBytes ctl1) (certificateTypeListBytes ctl2) ==> ctl1 = ctl2))
 let rec certificateTypeListBytes_is_injective ctl1 ctl2 =
   match ctl1, ctl2 with
   | [], [] -> ()
-  | hd::tl, hd'::tl' -> 
+  | hd::tl, hd'::tl' ->
     if certificateTypeListBytes ctl1 = certificateTypeListBytes ctl2 then (
       cut (Seq.equal (certTypeBytes hd @| certificateTypeListBytes tl) (certTypeBytes hd' @| certificateTypeListBytes tl'));
       lemma_append_inj (certTypeBytes hd) (certificateTypeListBytes tl) (certTypeBytes hd') (certificateTypeListBytes tl');
       cut(hd = hd');
       certificateTypeListBytes_is_injective tl tl'
     )
-  | _, _ -> () 
+  | _, _ -> ()
 
 #reset-options
 
@@ -963,17 +968,17 @@ let lemma_distinguishedNameListBytes_def (n:list dn{Cons? n /\ repr_bytes (lengt
 let lemma_distinguishedNameListBytes_def2 (n:list dn{Nil? n}) : Lemma (distinguishedNameListBytes n = empty_bytes) = ()
 
 (* TODO: port to Platform.Bytes *)
-assume val utf8_is_injective: s:string -> s':string -> 
+assume val utf8_is_injective: s:string -> s':string ->
   Lemma (requires (True))
 	(ensures (Seq.equal (utf8 s) (utf8 s') ==> s = s'))
 
-val distinguishedNameListBytes_is_injective: n1:list dn -> n2:list dn -> 
+val distinguishedNameListBytes_is_injective: n1:list dn -> n2:list dn ->
   Lemma (requires (True))
 	(ensures (Seq.equal (distinguishedNameListBytes n1) (distinguishedNameListBytes n2) ==> n1 = n2))
-let rec distinguishedNameListBytes_is_injective n1 n2 = 
+let rec distinguishedNameListBytes_is_injective n1 n2 =
   match n1, n2 with
   | [],[] -> ()
-  | hd::tl, hd'::tl' -> 
+  | hd::tl, hd'::tl' ->
       let payload1 = distinguishedNameListBytes n1 in
       let payload2 = distinguishedNameListBytes n2 in
       if payload1 = payload2 then (
@@ -984,7 +989,7 @@ let rec distinguishedNameListBytes_is_injective n1 n2 =
 	cut (forall b b'. {:pattern (b@|b')} (b@|b') = Seq.append b b');
 	Seq.lemma_eq_refl payload1 payload2;
 	cut (Seq.equal ((vlbytes 2 (utf8 hd)) @| (distinguishedNameListBytes tl))
-		       ((vlbytes 2 (utf8 hd')) @| (distinguishedNameListBytes tl')));	
+		       ((vlbytes 2 (utf8 hd')) @| (distinguishedNameListBytes tl')));
 	cut (Seq.equal (Seq.append (vlbytes 2 (utf8 hd)) (distinguishedNameListBytes tl))
 		       (Seq.append (vlbytes 2 (utf8 hd')) (distinguishedNameListBytes tl')));
         cut (Seq.index (vlbytes 2 (utf8 hd)) 0 = Seq.index payload1 0);
@@ -992,8 +997,8 @@ let rec distinguishedNameListBytes_is_injective n1 n2 =
         cut (Seq.index (vlbytes 2 (utf8 hd')) 0 = Seq.index payload2 0);
         cut (Seq.index (vlbytes 2 (utf8 hd')) 1 = Seq.index payload2 1);
 	cut (Seq.index payload1 0 = Seq.index payload2 0);
-        cut (Seq.index payload1 1 = Seq.index payload2 1);		
-	vlbytes_length_lemma 2 (utf8 hd) (utf8 hd');	
+        cut (Seq.index payload1 1 = Seq.index payload2 1);
+	vlbytes_length_lemma 2 (utf8 hd) (utf8 hd');
 	lemma_append_inj (vlbytes 2 (utf8 hd)) (distinguishedNameListBytes tl) (vlbytes 2 (utf8 hd')) (distinguishedNameListBytes tl');
 	distinguishedNameListBytes_is_injective tl tl';
 	lemma_vlbytes_inj 2 (utf8 hd) (utf8 hd');
@@ -1018,13 +1023,13 @@ let rec distinguishedNameListBytes_is_injective n1 n2 =
 
 //#set-options "--lax"
 
-val certificateRequestBytes_is_injective: c1:cr -> c2:cr -> 
+val certificateRequestBytes_is_injective: c1:cr -> c2:cr ->
   Lemma (requires (True))
 	(ensures (Seq.equal (certificateRequestBytes c1) (certificateRequestBytes c2) ==> c1 = c2))
 let certificateRequestBytes_is_injective c1 c2 =
   admit(); // JK: TODO
   if certificateRequestBytes c1 = certificateRequestBytes c2 then (
-    let ctb1 = certificateTypeListBytes c1.cr_cert_types in  
+    let ctb1 = certificateTypeListBytes c1.cr_cert_types in
     lemma_repr_bytes_values (length ctb1);
     let ctB1 = vlbytes 1 ctb1 in
     let saB1 = match c1.cr_sig_hash_algs with
@@ -1034,7 +1039,7 @@ let certificateRequestBytes_is_injective c1 c2 =
     lemma_repr_bytes_values (length dnb1);
     let dnB1 = vlbytes 2 dnb1 in
     let data1 = ctB1 @| saB1 @| dnB1 in
-    let ctb2 = certificateTypeListBytes c2.cr_cert_types in  
+    let ctb2 = certificateTypeListBytes c2.cr_cert_types in
     lemma_repr_bytes_values (length ctb2);
     let ctB2 = vlbytes 1 ctb2 in
     let saB2 = match c2.cr_sig_hash_algs with
@@ -1051,10 +1056,10 @@ let certificateRequestBytes_is_injective c1 c2 =
     assume (Seq.equal (Seq.slice data1 0 1) (Seq.slice ctB1 0 1));
     assume (Seq.equal (Seq.slice data2 0 1) (Seq.slice ctB2 0 1));
     vlbytes_length_lemma 1 ctb1 ctb2;
-    lemma_append_inj ctB1 (saB1 @| dnB1) ctB2 (saB2 @| dnB2)   
+    lemma_append_inj ctB1 (saB1 @| dnB1) ctB2 (saB2 @| dnB2)
   )
 
-val parseCertificateRequest: pv:protocolVersion -> data:bytes{repr_bytes(length data) <= 3} -> 
+val parseCertificateRequest: pv:protocolVersion -> data:bytes{repr_bytes(length data) <= 3} ->
                              Tot (result cr)
 let parseCertificateRequest version data =
     if length data >= 1 then
@@ -1066,7 +1071,7 @@ let parseCertificateRequest version data =
 	if List.Tot.length certTypeList < 256 then (
         if length data >= 2 then
             match version with
-            | TLS_1p2 -> 
+            | TLS_1p2 ->
             (match vlsplit 2 data with
             | Error(z) -> Error(z)
             | Correct  (x,y) ->
@@ -1074,7 +1079,7 @@ let parseCertificateRequest version data =
 	       lemma_repr_bytes_values (length x);
                match parseSigHashAlgs (vlbytes 2 x) with
                | Error(z) -> Error(z)
-               | Correct (sigAlgs) -> 
+               | Correct (sigAlgs) ->
 	       match vlparse 2 y with
 	       | Error(z) -> Error(z)
 	       | Correct(y) ->
@@ -1088,7 +1093,7 @@ let parseCertificateRequest version data =
                   cr_distinguished_names = distNamesList})
 		 else Error(AD_decode_error, perror __SOURCE_FILE__ __LINE__ "")
 	    end
-            else      
+            else
                Error(AD_decode_error, perror __SOURCE_FILE__ __LINE__ ""))
             | _ ->
                match parseDistinguishedNameList data [] with
@@ -1101,44 +1106,44 @@ let parseCertificateRequest version data =
                   cr_distinguished_names = distNamesList})
 		 else Error(AD_decode_error, perror __SOURCE_FILE__ __LINE__ "")
         else Error(AD_decode_error, perror __SOURCE_FILE__ __LINE__ "") )
-        else Error(AD_decode_error, perror __SOURCE_FILE__ __LINE__ "") 
+        else Error(AD_decode_error, perror __SOURCE_FILE__ __LINE__ "")
     else Error(AD_decode_error, perror __SOURCE_FILE__ __LINE__ "")
 
 let mk_certificateRequestBytes sign cs version =
     certificateRequestBytes (
     {cr_cert_types = defaultCertTypes sign cs;
-     cr_sig_hash_algs = (match version with 
-                         | TLS_1p2 -> Some (default_sigHashAlg version cs) 
+     cr_sig_hash_algs = (match version with
+                         | TLS_1p2 -> Some (default_sigHashAlg version cs)
                          | _ -> None);
-     cr_distinguished_names = []})                    
+     cr_distinguished_names = []})
 
 (** A.4.3 Client Authentication and Key Exchange Messages *)
 
 open CoreCrypto
-val kex_c_of_dh_key: CommonDH.key -> Tot kex_c
-let kex_c_of_dh_key kex = 
-  match kex with
-  | FFKey k -> KEX_C_DHE k.dh_public
-  | ECKey k -> KEX_C_ECDHE (ECGroup.serialize_point k.ec_params k.ec_point)
+val kex_c_of_dh_key: #g:CommonDH.group -> CommonDH.pre_share g -> Tot kex_c
+let kex_c_of_dh_key #g kex =
+  match g with
+  | CommonDH.FFDH g' -> KEX_C_DHE (CommonDH.serialize_raw #g kex)
+  | CommonDH.ECDH g' -> KEX_C_ECDHE (CommonDH.serialize_raw #g kex)
 
 (* JK: TODO: add the kex as an extra parameter, otherwise not injective *)
 val clientKeyExchangeBytes: protocolVersion -> cke -> Tot (b:bytes{hs_msg_bytes HT_client_key_exchange b})
-let clientKeyExchangeBytes pv cke = 
-  let kexB =              
+let clientKeyExchangeBytes pv cke =
+  let kexB =
     match pv,cke.cke_kex_c with
     | _,KEX_C_DHE b -> (
-      lemma_repr_bytes_values (length b); 
+      lemma_repr_bytes_values (length b);
       lemma_vlbytes_len 2 b;
       lemma_repr_bytes_values (length (vlbytes 2 b));
       vlbytes 2 b )
     | _,KEX_C_ECDHE b -> (
-      lemma_repr_bytes_values (length b); 
+      lemma_repr_bytes_values (length b);
       lemma_vlbytes_len 1 b;
       lemma_repr_bytes_values (length (vlbytes 1 b));
       vlbytes 1 b)
     | SSL_3p0,KEX_C_RSA(encpms) -> (lemma_repr_bytes_values (length encpms); encpms)
     | _,KEX_C_RSA(encpms) -> (
-      lemma_repr_bytes_values (length encpms); 
+      lemma_repr_bytes_values (length encpms);
       lemma_vlbytes_len 2 encpms;
       lemma_repr_bytes_values (length (vlbytes 2 encpms));
       vlbytes 2 encpms )
@@ -1151,7 +1156,7 @@ let clientKeyExchangeBytes pv cke =
 val clientKeyExchangeBytes_is_injective: pv:protocolVersion -> cke1:cke -> cke2:cke ->
   Lemma (requires (True))
 	(ensures (Seq.equal (clientKeyExchangeBytes pv cke1) (clientKeyExchangeBytes pv cke2) ==> cke1 = cke2))
-let clientKeyExchangeBytes_is_injective pv cke1 cke2 = 	
+let clientKeyExchangeBytes_is_injective pv cke1 cke2 =
   admit(); // JK: TODO, see comment above
   if clientKeyExchangeBytes pv cke1 = clientKeyExchangeBytes pv cke2 && pv = SSL_3p0 then (
     ()
@@ -1162,34 +1167,34 @@ let clientKeyExchangeBytes_is_injective pv cke1 cke2 =
 
 (* val parseClientKeyExchange: p:protocolVersion -> kex:kexAlg -> b:bytes{repr_bytes(length b) <= 3} ->  *)
 (*     Tot (result (cke:cke{Seq.equal (clientKeyExchangeBytes p cke) (messageBytes HT_client_key_exchange b)})) *)
-val parseClientKeyExchange: p:protocolVersion -> kex:kexAlg -> b:bytes{repr_bytes(length b) <= 3} -> 
+val parseClientKeyExchange: p:protocolVersion -> kex:kexAlg -> b:bytes{repr_bytes(length b) <= 3} ->
     Tot (result cke)
-let parseClientKeyExchange pv kex data = 
+let parseClientKeyExchange pv kex data =
   match pv,kex with
-  | _,Kex_DH -> 
-      if length data = 0 
+  | _,Kex_DH ->
+      if length data = 0
       then Correct({cke_kex_c = KEX_C_DH})
       else Error(AD_decode_error, perror __SOURCE_FILE__ __LINE__ "")
-  | _,Kex_DHE -> 
+  | _,Kex_DHE ->
       if length data >= 2
       then (match vlparse 2 data with
            | Error(z) -> Error(z)
            | Correct(y) -> (lemma_repr_bytes_values (length y); Correct({cke_kex_c = KEX_C_DHE y})))
       else Error(AD_decode_error, perror __SOURCE_FILE__ __LINE__ "")
-  | _,Kex_ECDHE -> 
+  | _,Kex_ECDHE ->
       if length data >= 1
       then (match vlparse 1 data with
            | Error(z) -> Error(z)
            | Correct(y) -> (lemma_repr_bytes_values (length y); Correct({cke_kex_c = KEX_C_ECDHE y})))
       else Error(AD_decode_error, perror __SOURCE_FILE__ __LINE__ "")
-  | SSL_3p0,Kex_RSA -> 
+  | SSL_3p0,Kex_RSA ->
       if length data < 4096 then
          (lemma_repr_bytes_values (length data); Correct({cke_kex_c = KEX_C_RSA data}))
       else Error(AD_decode_error, perror __SOURCE_FILE__ __LINE__ "")
-  | _,Kex_RSA  -> 
+  | _,Kex_RSA  ->
         if length data >= 2 then
             match vlparse 2 data with
-            | Correct (encPMS) -> 
+            | Correct (encPMS) ->
 	      if length encPMS < 4096 then (lemma_repr_bytes_values (length encPMS); correct({cke_kex_c = KEX_C_RSA encPMS}))
 	      else Error(AD_decode_error, perror __SOURCE_FILE__ __LINE__ "")
             | Error(z) -> Error(z)
@@ -1200,20 +1205,20 @@ let parseClientKeyExchange pv kex data =
 open CoreCrypto
 
 val kex_s_to_bytes: kex_s -> Tot (b:bytes{length b < 16777216 - 65536}) // JK: required for serverKeyExxchangeBytes
-let kex_s_to_bytes kex = 
+let kex_s_to_bytes kex =
   admit(); // JK: TODO
   match kex with
-  | KEX_S_DHE k -> CommonDH.serialize k 
+  | KEX_S_DHE (|g, k|) -> CommonDH.serialize #g k
   | KEX_S_RSA pk -> (*TODO: Ephemeral RSA*) empty_bytes
 
 (* JK: TODO, or rewrite the functions altogether *)
-assume val commonDH_serialize_is_injective: k1:CommonDH.key -> k2:CommonDH.key -> 
+assume val commonDH_serialize_is_injective: #g:CommonDH.group -> k1:CommonDH.pre_share g -> k2:CommonDH.pre_share g ->
   Lemma (requires (True))
 	(ensures (Seq.equal (CommonDH.serialize k1) (CommonDH.serialize k2) ==> k1 = k2))
 
 (* JK: TODO: missing the proper serialization for RSA so not injective for now *)
 (* Actually false for now *)
-assume val kex_s_to_bytes_is_injective: k1:kex_s -> k2:kex_s -> 
+assume val kex_s_to_bytes_is_injective: k1:kex_s -> k2:kex_s ->
   Lemma (requires (True))
 	(ensures (Seq.equal (kex_s_to_bytes k1) (kex_s_to_bytes k2) ==> k1 = k2))
 
@@ -1224,9 +1229,9 @@ let serverKeyExchangeBytes ske =
     lemma_repr_bytes_values (length payload);
     messageBytes HT_server_key_exchange payload
 
-(* JK: TODO, currently not injective and missing an extra argument compared to the 
+(* JK: TODO, currently not injective and missing an extra argument compared to the
    parsing function: the kex algorithm *)
-assume val serverKeyExchangeBytes_is_injective: s1:ske -> s2:ske -> 
+assume val serverKeyExchangeBytes_is_injective: s1:ske -> s2:ske ->
   Lemma (requires (True))
 	(ensures (Seq.equal (serverKeyExchangeBytes s1) (serverKeyExchangeBytes s2) ==> s1 = s2))
 (* let serverKeyExchangeBytes_is_injective s1 s2 =  *)
@@ -1244,20 +1249,20 @@ assume val serverKeyExchangeBytes_is_injective: s1:ske -> s2:ske ->
 (* val parseServerKeyExchange: kex:kexAlg -> b:bytes{repr_bytes(length b) <= 3} ->  *)
 (*     Tot (result (s:ske{Seq.equal (serverKeyExchangeBytes s) (messageBytes HT_server_key_exchange b)})) *)
 val parseServerKeyExchange: kex:kexAlg -> b:bytes{repr_bytes(length b) <= 3} -> Tot (result ske)
-let parseServerKeyExchange kex payload : result ske = 
+let parseServerKeyExchange kex payload : result ske =
     match kex with
     | Kex_DH -> Error(AD_decode_error, perror __SOURCE_FILE__ __LINE__ "")
     | Kex_RSA -> Error(AD_decode_error, perror __SOURCE_FILE__ __LINE__ "")
-    | Kex_DHE -> 
-       (match CommonDH.parse_partial payload false with
-	| Correct (k,sign) -> 
+    | Kex_DHE ->
+       (match CommonDH.parse_partial false payload with
+	| Correct (k,sign) ->
 	  if length sign < 65536 then
           Correct ({ske_kex_s = KEX_S_DHE k;
                     ske_sig = sign})
 	  else Error(AD_decode_error, perror __SOURCE_FILE__ __LINE__ "")
         | Error z -> Error z)
-    | Kex_ECDHE -> 
-       (match CommonDH.parse_partial payload true with
+    | Kex_ECDHE ->
+       (match CommonDH.parse_partial true payload with
 	| Correct (k,sign) ->
 	  if length sign < 65536 then
           Correct ({ske_kex_s = KEX_S_DHE k;
@@ -1267,39 +1272,39 @@ let parseServerKeyExchange kex payload : result ske =
 
 (* Certificate Verify *)
 val certificateVerifyBytes: cv -> Tot (b:bytes{hs_msg_bytes HT_certificate_verify b})
-let certificateVerifyBytes cv = 
+let certificateVerifyBytes cv =
     lemma_repr_bytes_values (length cv.cv_sig);
     messageBytes HT_certificate_verify cv.cv_sig
 
-val certificateVerifyBytes_is_injective: c1:cv -> c2:cv -> 
+val certificateVerifyBytes_is_injective: c1:cv -> c2:cv ->
   Lemma (requires (True))
 	(ensures (Seq.equal (certificateVerifyBytes c1) (certificateVerifyBytes c2) ==> c1 = c2))
-let certificateVerifyBytes_is_injective c1 c2 = 
+let certificateVerifyBytes_is_injective c1 c2 =
   if certificateVerifyBytes c1 = certificateVerifyBytes c2 then (
     lemma_repr_bytes_values (length c1.cv_sig);
-    lemma_repr_bytes_values (length c2.cv_sig);    
+    lemma_repr_bytes_values (length c2.cv_sig);
     messageBytes_is_injective HT_certificate_verify c1.cv_sig HT_certificate_verify c2.cv_sig
   )
 
-(* JK: FIXME: information on data's length is redundant, but simpler for now to have both 
+(* JK: FIXME: information on data's length is redundant, but simpler for now to have both
    in the spec *)
 val parseCertificateVerify: data:bytes{length data < 65536 /\ repr_bytes(length data) <= 3} ->
     Tot (result (c:cv{Seq.equal (certificateVerifyBytes c) (messageBytes HT_certificate_verify data)}))
-let parseCertificateVerify data = 
+let parseCertificateVerify data =
     correct ({cv_sig = data})
 
 val finishedBytes: fin -> Tot (b:bytes{hs_msg_bytes HT_finished b})
-let finishedBytes fin = 
+let finishedBytes fin =
     lemma_repr_bytes_values (length fin.fin_vd);
     messageBytes HT_finished fin.fin_vd
 
-val finishedBytes_is_injective: f1:fin -> f2:fin -> 
+val finishedBytes_is_injective: f1:fin -> f2:fin ->
   Lemma (requires (True))
 	(ensures (Seq.equal (finishedBytes f1) (finishedBytes f2) ==> f1 = f2))
-let finishedBytes_is_injective f1 f2 = 
+let finishedBytes_is_injective f1 f2 =
   if finishedBytes f1 = finishedBytes f2 then (
     lemma_repr_bytes_values (length f1.fin_vd);
-    lemma_repr_bytes_values (length f2.fin_vd);    
+    lemma_repr_bytes_values (length f2.fin_vd);
     messageBytes_is_injective HT_finished f1.fin_vd HT_finished f2.fin_vd
   )
 
@@ -1308,7 +1313,7 @@ let finishedBytes_is_injective f1 f2 =
 
 val parseFinished: data:bytes{length data < 65536 /\ repr_bytes(length data)<=3} ->
     Tot (result(f:fin{Seq.equal (finishedBytes f) (messageBytes HT_finished data)}))
-let parseFinished data = 
+let parseFinished data =
     Correct ({fin_vd = data})
 
 (* Session ticket *)
@@ -1318,10 +1323,10 @@ let sessionTicketBytes sticket =
     lemma_repr_bytes_values (length payload);
     messageBytes HT_session_ticket payload
 
-val sessionTicketBytes_is_injective: s1:sticket -> s2:sticket -> 
+val sessionTicketBytes_is_injective: s1:sticket -> s2:sticket ->
   Lemma (requires (True))
 	(ensures (Seq.equal (sessionTicketBytes s1) (sessionTicketBytes s2) ==> s1 = s2))
-let sessionTicketBytes_is_injective s1 s2 = 
+let sessionTicketBytes_is_injective s1 s2 =
   if sessionTicketBytes s1 = sessionTicketBytes s2 then (
     let payload1 = s1.sticket_ticket_lifetime_hint @| s1.sticket_ticket in
     let payload2 = s2.sticket_ticket_lifetime_hint @| s2.sticket_ticket in
@@ -1331,9 +1336,9 @@ let sessionTicketBytes_is_injective s1 s2 =
     lemma_append_inj s1.sticket_ticket_lifetime_hint s1.sticket_ticket s2.sticket_ticket_lifetime_hint s2.sticket_ticket
   )
 
-val parseSessionTicket: b:bytes{repr_bytes(length b) <= 3} -> 
+val parseSessionTicket: b:bytes{repr_bytes(length b) <= 3} ->
     Tot (result (s:sticket{Seq.equal (sessionTicketBytes s) (messageBytes HT_session_ticket b)}))
-let parseSessionTicket payload  = 
+let parseSessionTicket payload  =
   if length payload >= 4 && length payload < 65542 then
     let (lifetime_hint, ticket) = split payload 4 in
     Correct({sticket_ticket_lifetime_hint = lifetime_hint; sticket_ticket = ticket})
@@ -1350,16 +1355,16 @@ let helloRetryRequestBytes hrr =
   lemma_repr_bytes_values (length data);
   messageBytes HT_hello_retry_request data
 
-val namedGroupBytes_is_injective: n1:namedGroup -> n2:namedGroup -> 
+val namedGroupBytes_is_injective: n1:namedGroup -> n2:namedGroup ->
   Lemma (requires (True))
 	(ensures (Seq.equal (namedGroupBytes n1) (namedGroupBytes n2) ==> n1 = n2))
-let namedGroupBytes_is_injective n1 n2 = 
+let namedGroupBytes_is_injective n1 n2 =
   if namedGroupBytes n1 = namedGroupBytes n2 then pinverse_namedGroup (namedGroupBytes n1)
 
-val helloRetryRequestBytes_is_injective: h1:hrr -> h2:hrr -> 
+val helloRetryRequestBytes_is_injective: h1:hrr -> h2:hrr ->
   Lemma (requires (True))
 	(ensures (Seq.equal (helloRetryRequestBytes h1) (helloRetryRequestBytes h2) ==> h1 == h2))
-let helloRetryRequestBytes_is_injective h1 h2 = 
+let helloRetryRequestBytes_is_injective h1 h2 =
   if helloRetryRequestBytes h1 = helloRetryRequestBytes h2 then (
     let pv1 = versionBytes h1.hrr_protocol_version in
     let cs_bytes1 = cipherSuiteBytes h1.hrr_cipher_suite in
@@ -1385,19 +1390,19 @@ let helloRetryRequestBytes_is_injective h1 h2 =
 
 (* TODO: inversion lemmas *)
 val parseHelloRetryRequest: bytes -> Tot (result hrr)
-let parseHelloRetryRequest b = 
-  if length b >= 4 then 
+let parseHelloRetryRequest b =
+  if length b >= 4 then
     let pv, cs, data = split2 b 2 2 in
     (match TLSConstants.parseVersion pv with
-    | Correct(pv) -> 
+    | Correct(pv) ->
       (match parseCipherSuite cs with
-      | Correct(cs) -> 
+      | Correct(cs) ->
 	if length data >= 2 then
 	  let ng, data = split data 2 in
 	  (match parseNamedGroup ng with
 	  | Correct(ng) ->
 	    (match parseExtensions Server data with
-	    | Correct(exts) -> 
+	    | Correct(exts) ->
 	      if List.Tot.length exts < 256 then
 	      Correct ({ hrr_protocol_version = pv;
 			hrr_cipher_suite = cs;
@@ -1407,7 +1412,7 @@ let parseHelloRetryRequest b =
 	    | Error(z) -> Error(z))
 	  | Error(z) -> Error(z))
 	else Error (AD_decode_error, perror __SOURCE_FILE__ __LINE__ "Wrong hello retry request format")
-      | Error(z) -> Error(z))  
+      | Error(z) -> Error(z))
     | Error(z) -> Error(z))
   else Error (AD_decode_error, perror __SOURCE_FILE__ __LINE__ "Wrong hello retry request format")
 
@@ -1419,7 +1424,7 @@ let encryptedExtensionsBytes ee =
     let payload = extensionsBytes Server ee.ee_extensions in
     messageBytes HT_encrypted_extensions payload
 
-val encryptedExtensionsBytes_is_injective: e1:valid_ee -> e2:valid_ee -> 
+val encryptedExtensionsBytes_is_injective: e1:valid_ee -> e2:valid_ee ->
   Lemma (requires (True))
 	(ensures (Seq.equal (encryptedExtensionsBytes e1) (encryptedExtensionsBytes e2) ==> e1 == e2))
 let encryptedExtensionsBytes_is_injective e1 e2 =
@@ -1429,15 +1434,15 @@ let encryptedExtensionsBytes_is_injective e1 e2 =
   extensionsBytes_is_injective Server e1.ee_extensions e2.ee_extensions
 
 (* JK : TODO *)
-assume val lemma_extensionsBytes_length: r:role -> b:bytes -> 
+assume val lemma_extensionsBytes_length: r:role -> b:bytes ->
   Lemma (requires (True))
 	(ensures (Correct? (parseExtensions r b) ==> length (extensionsBytes r (Correct?._0 (parseExtensions r b))) = length b))
 
 (* val parseEncryptedExtensions: b:bytes{repr_bytes(length b) <= 3} ->  *)
 (*     Tot (result (s:valid_ee{Seq.equal (encryptedExtensionsBytes s) (messageBytes HT_encrypted_extensions b)})) *)
-val parseEncryptedExtensions: b:bytes{repr_bytes(length b) <= 3} -> 
+val parseEncryptedExtensions: b:bytes{repr_bytes(length b) <= 3} ->
     Tot (result valid_ee)
-let parseEncryptedExtensions payload  = 
+let parseEncryptedExtensions payload  =
   match parseExtensions Server payload with
   | Error(z) -> Error(z)
   | Correct(exts) -> if List.Tot.length exts < 256 then (
@@ -1456,10 +1461,10 @@ let nextProtocolBytes np =
   lemma_repr_bytes_values (length (selected_protocol @| padding));
   messageBytes HT_next_protocol (selected_protocol @| padding)
 
-val nextProtocolBytes_is_injective: np1:np -> np2:np -> 
+val nextProtocolBytes_is_injective: np1:np -> np2:np ->
   Lemma (requires (True))
 	(ensures (Seq.equal (nextProtocolBytes np1) (nextProtocolBytes np2) ==> np1 = np2))
-let nextProtocolBytes_is_injective np1 np2 = 
+let nextProtocolBytes_is_injective np1 np2 =
   if nextProtocolBytes np1 = nextProtocolBytes np2 then (
     lemma_repr_bytes_values (length (np1.np_selected_protocol));
     lemma_repr_bytes_values (length (np1.np_padding));
@@ -1509,7 +1514,7 @@ let valid_hs_msg: Type0 = msg:hs_msg{
   /\ (Certificate? msg ==> length (Cert.certificateListBytes (Certificate?._0 msg).crt_chain) < 16777212)}
 
 val handshakeMessageBytes: pv:option protocolVersion -> msg:valid_hs_msg{associated_to_pv pv msg}  -> Tot (b:bytes{exists (ht:handshakeType). hs_msg_bytes ht b})
-let handshakeMessageBytes pvo hs = 
+let handshakeMessageBytes pvo hs =
     match hs,pvo with
     | ClientHello(ch),_-> clientHelloBytes ch
     | ServerHello(sh),_-> serverHelloBytes sh
@@ -1527,7 +1532,7 @@ let handshakeMessageBytes pvo hs =
     (* | ServerConfiguration(sc),_-> serverConfigurationBytes sc *)
     | NextProtocol(n),_->  nextProtocolBytes n
 
-val splitHandshakeMessage: b:bytes{exists (ht:handshakeType). hs_msg_bytes ht b} -> 
+val splitHandshakeMessage: b:bytes{exists (ht:handshakeType). hs_msg_bytes ht b} ->
   Tot (t:(handshakeType * bytes){repr_bytes (length (snd t)) <= 3 /\ b = (htBytes (fst t) @| (vlbytes 3 (snd t)))})
 let splitHandshakeMessage b =
   let htbytes, payload = split b 1 in
@@ -1543,7 +1548,7 @@ let splitHandshakeMessage b =
 #reset-options "--z3rlimit 100"
 //#set-options "--lax"
 
-val handshakeMessageBytes_is_injective: pv:option protocolVersion -> msg1:valid_hs_msg{associated_to_pv pv msg1} -> msg2:valid_hs_msg{associated_to_pv pv msg2} -> 
+val handshakeMessageBytes_is_injective: pv:option protocolVersion -> msg1:valid_hs_msg{associated_to_pv pv msg1} -> msg2:valid_hs_msg{associated_to_pv pv msg2} ->
   Lemma (requires (True))
 	(ensures (Seq.equal (handshakeMessageBytes pv msg1) (handshakeMessageBytes pv msg2) ==> msg1 = msg2))
 let handshakeMessageBytes_is_injective pv msg1 msg2 =
@@ -1573,7 +1578,7 @@ let handshakeMessageBytes_is_injective pv msg1 msg2 =
   )
 
 val handshakeMessagesBytes: pv:option protocolVersion -> list (msg:valid_hs_msg{associated_to_pv pv msg}) -> Tot bytes
-let rec handshakeMessagesBytes pv hsl = 
+let rec handshakeMessagesBytes pv hsl =
     match hsl with
     | [] -> empty_bytes
     | h::t -> (handshakeMessageBytes pv h) @| (handshakeMessagesBytes pv t)
@@ -1584,10 +1589,10 @@ let lemma_handshakeMessagesBytes_def (pv:option protocolVersion) (li:list (msg:v
 
 let lemma_handshakeMessagesBytes_def2 (pv:option protocolVersion) (li:list (msg:valid_hs_msg{associated_to_pv pv msg}){Nil? li}) : Lemma (handshakeMessagesBytes pv li = empty_bytes) = ()
 
-val lemma_handshakeMessageBytes_aux: pv:option protocolVersion -> msg1:valid_hs_msg{associated_to_pv pv msg1} -> msg2:valid_hs_msg{associated_to_pv pv msg2} -> 
+val lemma_handshakeMessageBytes_aux: pv:option protocolVersion -> msg1:valid_hs_msg{associated_to_pv pv msg1} -> msg2:valid_hs_msg{associated_to_pv pv msg2} ->
   Lemma (requires (let b1 = handshakeMessageBytes pv msg1 in
 		       let b2 = handshakeMessageBytes pv msg2 in
-		       length b2 >= length b1 
+		       length b2 >= length b1
 		       /\ Seq.equal b1 (Seq.slice b2 0 (length b1))))
 	(ensures (Seq.equal (handshakeMessageBytes pv msg1) (handshakeMessageBytes pv msg2)))
 
@@ -1617,10 +1622,10 @@ let lemma_handshakeMessageBytes_aux pv msg1 msg2 =
 
 #reset-options
 
-let lemma_aux_1 (a:bytes) (b:bytes) (c:bytes) (d:bytes) : Lemma 
+let lemma_aux_1 (a:bytes) (b:bytes) (c:bytes) (d:bytes) : Lemma
   (requires (Seq.equal (a @| b) (c @| d)))
   (ensures ((length a >= length c ==> Seq.equal (Seq.slice a 0 (length c)) c)
-	    /\ (length a < length c ==> Seq.equal (Seq.slice c 0 (length a)) a))) 
+	    /\ (length a < length c ==> Seq.equal (Seq.slice c 0 (length a)) a)))
  = if length a >= length c then (
      cut (Seq.equal (a @| b) (c @| d));
      cut (forall (i:nat). {:pattern (Seq.index (a@|b) i) \/ (Seq.index (c@|d) i)} i < length (a@|b) ==> Seq.index (a@|b) i = Seq.index (c@|d) i);
@@ -1646,7 +1651,7 @@ let lemma_aux_2 (pv:option protocolVersion) (l:list (msg:valid_hs_msg{associated
 let lemma_aux_3 (b:bytes) (b':bytes) : Lemma (requires (length b <> length b'))
 					    (ensures (~(Seq.equal b b'))) = ()
 
-val handshakeMessagesBytes_is_injective: pv:option protocolVersion -> l1:list (msg:valid_hs_msg{associated_to_pv pv msg}) -> l2:list (msg:valid_hs_msg{associated_to_pv pv msg}) -> 
+val handshakeMessagesBytes_is_injective: pv:option protocolVersion -> l1:list (msg:valid_hs_msg{associated_to_pv pv msg}) -> l2:list (msg:valid_hs_msg{associated_to_pv pv msg}) ->
   Lemma (requires (True))
 	(ensures (Seq.equal (handshakeMessagesBytes pv l1) (handshakeMessagesBytes pv l2) ==> l1 = l2))
 let rec handshakeMessagesBytes_is_injective pv l1 l2 =
@@ -1664,7 +1669,7 @@ let rec handshakeMessagesBytes_is_injective pv l1 l2 =
       if payload1 = payload2 then (
 	cut (Seq.equal (Seq.append (handshakeMessageBytes pv hd) (handshakeMessagesBytes pv tl))
 		       (Seq.append (handshakeMessageBytes pv hd') (handshakeMessagesBytes pv tl')));
-	cut (Seq.equal ((handshakeMessageBytes pv hd) @| (handshakeMessagesBytes pv tl)) ((handshakeMessageBytes pv hd') @| (handshakeMessagesBytes pv tl')));	
+	cut (Seq.equal ((handshakeMessageBytes pv hd) @| (handshakeMessagesBytes pv tl)) ((handshakeMessageBytes pv hd') @| (handshakeMessagesBytes pv tl')));
 	if length (handshakeMessageBytes pv hd) >= length (handshakeMessageBytes pv hd')
 	then (
 	  lemma_aux_1 (handshakeMessageBytes pv hd) (handshakeMessagesBytes pv tl) (handshakeMessageBytes pv hd') (handshakeMessagesBytes pv tl');
@@ -1691,7 +1696,7 @@ let rec handshakeMessagesBytes_is_injective pv l1 l2 =
     )
 
 val string_of_handshakeMessage: hs_msg -> Tot string
-let string_of_handshakeMessage hs = 
+let string_of_handshakeMessage hs =
     match hs with
     | ClientHello(ch) -> "ClientHello"
     | ServerHello(sh) -> "ServerHello"
@@ -1711,7 +1716,7 @@ let string_of_handshakeMessage hs =
 
 (* val parseHandshakeMessage: option protocolVersion -> option kexAlg -> handshakeType -> b:bytes{repr_bytes (length b) <= 3} -> Tot (result hs_msg) *)
 val parseHandshakeMessage: option protocolVersion -> option kexAlg -> ht:handshakeType -> b:bytes{repr_bytes (length b) <= 3} -> Tot (result hs_msg)
-let parseHandshakeMessage pv kex hstype pl = 
+let parseHandshakeMessage pv kex hstype pl =
   if length pl < 16777216 then (
     lemma_repr_bytes_values (length pl);
     match hstype,pv,kex with
@@ -1734,7 +1739,6 @@ let parseHandshakeMessage pv kex hstype pl =
     | HT_next_protocol,_,_       -> mapResult NextProtocol (parseNextProtocol pl)
     | HT_finished,_,_            -> (if length pl < 65536 then mapResult Finished (parseFinished pl)
       else Error(AD_decode_error, perror __SOURCE_FILE__ __LINE__ "") )
-    | _ -> Error(AD_decode_error, perror __SOURCE_FILE__ __LINE__ "") 
+    | _ -> Error(AD_decode_error, perror __SOURCE_FILE__ __LINE__ "")
     )
-  else  Error(AD_decode_error, perror __SOURCE_FILE__ __LINE__ "") 
-   
+  else  Error(AD_decode_error, perror __SOURCE_FILE__ __LINE__ "")
