src/tls/ODH.fst
@@ -1,74 +1,3 @@
-(**************************************************************************)
-(** A simple idealization of CommonDH that records honestly generated shares *)
-module DH
-module MS = MonotoneSet
-
-type group
-val strongGroup: g:group -> GTot bool
-type share (g:group)
-type keyshare (g:group)
-val pubshare: g:group -> s:keyshare g -> share g
-
-(* Global log of honestly generated DH shares *)
-private let dh_region:rgn = new_region tls_tables_region
-private type share_table =
-  (if Flags.ideal_kef then
-    MS.t dh_region (g:group & s:share g) grows
-  else
-    ())
-
-abstract let share_log: share_table =
-  (if Flags.ideal_kef then
-    MS.alloc #dh_region #(g:group & s:share g) #grows
-  else
-    ())
-
-abstract type honest_share (#g:group) (s:share g) =
-  Flags.ideal_kef ==> witnessed (MS.contains share_log (g,s))
-
-let is_honest (#g:group) (s:share g) : ST bool
-  (requires (fun h0 -> True))
-  (ensures (fun h0 b h1 ->
-    modifies_none h0 h1 /\
-    b <==> honest_share s)) =
-  if Flags.ideal_kef then
-    Some? (MS.lookup share_log (g,s))
-  else None
-
-let keygen (g:group) : ST (s:keyshare g)
-  (requires (fun h0 -> True))
-  (ensures (fun h0 s h1 ->
-    if Flags.ideal_kef then
-      modifies_one dh_region h0 h1 /\
-      MR.m_sel h1 share_log == Set.union (MR.m_sel h0 share_log) (Set.singleton (g, pubshare s)) /\
-      witnessed (MS.contains share_log (g, pubshare s))
-    else h0 = h1))
-  =
-  let ks = CommonDH.keygen g in
-  if Flags.ideal_kef then
-   begin
-    MR.m_recall share_log;
-    MS.append share_log (g, pubshare ks);
-    witness share_log (MS.contains share_log (g, pubshare ks))
-   end;
-  ks
-
-let initiator (#g:group) (si:keyshare g) (sr:share g)
-  : St (keyshare g * secret g) =
-  CommonDH.initiator si sr
-
-let responder (#g:group) (si:share g)
-  : St (secret g) =
-  CommonDH.responder si
-
-let coerce (g:group) (b:mlbytes (CommonDH.explen g)) : Tot (s:share g{hasExp s}) =
-  CommonDH.exponentiate g (CommonDH.generator g) exp
-let parse (g:group) (b:mlbytes (CommonDH.sharelen g)) : Tot (result (share g)) =
-  CommonDH.parse g b
-let serialize (#g:group) (s:share g) : Tot (b:mlbytes (CommonDH.sharelen g))
-  (ensures (parse g b = s))
-  = CommonDH.serialize g s
-
 ////////////////////////////////////////////////////////////////////////////////
 
 module KEF
@@ -88,10 +17,36 @@ type kef_type =
 
 // Instance indexing. TODO: check that there is no possible collision
 // between DH and DH_PSK instances
-type id = {
+type pre_id = {
   alg: kefalg;
   kef_type: kef_type;
 }
+
+let safety_table =
+  (if Flags.ideal_kef then
+    MM.alloc #kef_region #id #(fun i -> bool) #(fun _ -> True)
+  else unit)
+
+type registered (i:id) =
+  (if Flags.ideal_kef then
+    MR.witnessed (MM.defined safety_table i)
+  else True)
+
+type id = i:pre_id{registered i}
+
+type safeId (i:id) =
+  (if Flags.ideal_kef then
+    MR.witnessed (MM.contains KEF.safe_table i true)
+  else False)
+
+let is_safe (i:id) : ST bool
+  (requires (fun h0 -> True))
+  (ensures (fun h0 b h1 -> modifies_none h0 h1 /\ b <==> safeId i))
+  =
+  Flags.ideal_KEF_PRF &&
+  (match i.kef_type with
+  | PSK pski -> PSK.safePSK pski
+  | DH_PSK esId _ _ _ -> honest_esId esId)
 
 type dhrole =
   | Initiator
@@ -198,42 +153,24 @@ let extract (i:id) (ir:role i) (ikm:ikm i ir) (salt:salt i)
 
 ///////////////////////////////////////////
 
+// Middle extraction modeled as a PRF keyed by the extraction salt
 module KEF_PRF
 open KEF
 
-type id = i:id{PSK? i.kef_type \/ ZERO? i.kef_type \/ DH_PSK? i.kef_type}
+type id = i:id{PSK? i.kef_type \/ DH_PSK? i.kef_type}
 
-let safeId (i:id) =
-  (match i.kef_type with
-  | PSK pski -> PSK.safePSK pski
-  | ZERO hsId -> honest_hsId hsId
-  | DH_PSK esId _ _ _ -> honest_esId esId)
+type prf_key (i:id) = salt i
 
-(** Type of values used to key the PRF *)
-type prf_key (i:id) =
-  (match i.kef_type with
-  | PSK pski -> PSK.psk pski
-  | ZERO hsId -> expanded_secret (HandshakeSecretID hsId)
-  | DH_PSK esId _ _ _ -> expanded_secret (EarlySecretID esId))
-
-let prf_keylen (i:id) =
-  (match i.kef_type with
-  | PSK pski -> PSK.psklen pski
-  | ZERO hsId -> hashlen (hsId_hash hsId)
-  | DH_PSK esId _ _ _ -> hashlen (esId_hash esId)
-
-(** Type of the domain of the keyed PRF *)
 type prf_domain (i:id) =
   (match i.kef_type with
-  | PSK _ -> unit
-  | ZERO _ -> unit
-  | DH_PSK _ _ _ _ -> bytes
+  | PSK _ -> unit // Can only extract 0 in pure PSK
+  | DH_PSK _ g _ _ -> DH.secret g
 
 type prf_range (i:id) (d:domain i) = extracted_secret i
 
 (* Compact style: only allocate log for idealized instances *)
 type log (i:id) (r:rgn) =
-  (if Flags.ideal_kef /\ safeId i then
+  (if safeId i then
     MM.t r (prf_domain i) (prf_range i)
   else
     unit)
@@ -241,40 +178,33 @@ type log (i:id) (r:rgn) =
 type state (i:id) =
   | State:
      r:rgn ->
-     key: prf_key i
+     key: prf_key i ->
      log: log i r ->
      state i
 
-let create (i:id) (parent:rgn) : ST (state i)
-  (requires (fun h0 -> safeId i))
+let create (i:id) (parent:rgn) (key:prf_key i) : ST (state i)
+  (requires (fun h0 -> True))
   (ensures (fun h0 st h1 ->
     modifies_none h0 h1 /\
     extends st.r parent /\
     stronger_fresh_region st.r h0 h1 /\
-    if Flags.ideal_kef then
+    if safeId i then
       h1 `contains` st.log /\
       MM.m_sel h1 st.log == MM.empty_map
     else
       True))
   =
   let r = new_region parent in
-  let key : prf_key i = Bytes.random (prf_keylen i) in
   let log =
-    if Flags.ideal_kef then
+    if is_safe i then
       MM.alloc #r #(prf_domain i) #(prf_range i) #grows
     else () in
   State r key log
 
-let coerce (i:id) (r:rgn) (k:prf_key i) : ST (state i)
-  (requires (fun h0 -> ~(safeId i)))
-  (ensures (fun h0 st h1 -> h0 = h1))
-  =
-  State r k ()
-
 let extract (i:id) (st:state i) (v:prf_domain i) : ST (prf_range i v)
   (requires (fun h0 -> True))
   (ensures (fun h0 r h1 ->
-    if Flags.ideal_kef /\ safeId i then
+    if safeId i then
       (match MM.sel (MR.m_sel h0 st.log) v with
       | None ->
         modifies_one st.r h0 h1 /\
@@ -287,7 +217,7 @@ let extract (i:id) (st:state i) (v:prf_domain i) : ST (prf_range i v)
       h0 = h1
   ))
   =
-  if Flags.ideal_kef && safeId i then
+  if is_safe i then
     (match MM.lookup st.log v with
     | Some r -> r
     | None ->
@@ -297,10 +227,9 @@ let extract (i:id) (st:state i) (v:prf_domain i) : ST (prf_range i v)
   else
     let concrete_v =
       (match i.kef_type with
-      | PSK pskid -> zH (PSK.pskid_hash pskid // TODO move from KeySchedule
-      | ZERO hsId -> zH (hsId_hash hsId)
+      | PSK pskid -> zH (PSK.pskid_hash pskid)
       | DH_PSK _ _ _ _ -> v) in
-    Hacl.KEF.extract (i.alg) st.key concrete_v // e.g. HKDF
+    Hacl.KEF.extract (i.alg) concrete_v st.key // st.key is the salt
 
 module KEF_PRF_ODH
 
@@ -308,12 +237,8 @@ type id = i:KEF.id{DH? i.kef_type \/ DH_PSK? i.kef_type}
 
 let ishare_of_id (i:id) =
   match i.kef_type with
-  | DH g si -> (g, si)
-  | DH_PSK _ g si -> (g, si)
-
-inline_for_extraction let safeId (i:id) : Tot bool =
-  let (g, si, sr) = shares_of_id i in
-  Flags.ideal_kef && DH.strongGroup g && DH.honest_share si && DH.honest_share sr
+  | DH g si -> (| g, si |)
+  | DH_PSK _ g si -> (| g, si |)
 
 type salt (i:id) =
   (match i.kef_type with
@@ -333,180 +258,104 @@ type log (i:id) (r:rgn) =
   else
     unit)
 
-type odh_key (i:id) (ir:dhrole) =
-  (let g, si = ishare_of_id i in
-  if ir = Initiator then
-    ks:DH.keyshare g{DH.pubshare ks = si}
-   else
-    sr:DH.keyshare g{honest_share (pubshare ks)} * DH.secret (g,si,pubshare sr) * n:salt i)
-
 type state (i:id) (ir:dhrole) =
   | State:
     r: rgn ->
-    key: odh_key i ir ->
-    log: log i r ->
+    key: ikm i ir -> // initiator keyshare or responder salt
+    log: log i r -> // Map of responder share and salt to extracted secrets
+    // The responder share used by the initiator.
+    initiator_responder: rref r (o:option (odh_index i){is_Some o ==> MR.witnessed (MM.defined log (Some.v o))}) ->
     state i
 
 type odh_initiator (i:id) = state i Initiator
 type odh_responder (i:id) = state i Responder
 
-let create (i:id) (ir:role i) (ikm:ikm i ir) : ST (state i ir)
+let create (i:id) (ir:role i) (parent:rgn) (ikm:ikm i ir) : ST (state i ir)
   (requires (fun h0 -> True))
-  (ensures (fun h0 st h1 -> True))
+  (ensures (fun h0 st h1 ->
+    modifies_none h0 h1 /\
+    stronger_fresh_region r parent /\
+    empty_log (MM.sel h1 st.log) /\
+    is_None (sel h1 st.initiator_responder)))
   =
   let r = new_region parent in
   let (g, si) = ishare_of_id i in
   let log =
-    if Flags.ideal_kef && DH.is_honest si then
-      MM.alloc #r #(odh_index i) #(odh_extracted i) #grows
+    if is_safe i then
+      MM.alloc #r #(odh_index i) #(odh_extracted i) #(fun _ -> True)
     else () in
-  let key = match ir with
-    | Initiator -> ikm
-    | Responder ->
-      let n = ikm in
-      let sr, secret = DH.responder g si in
-      (sr, secret, n)
-    in
-  State r key log
+  let initiator_responder = ralloc r None in
+  State r key log initiator_responder
 
-let extract_responder (i:id) (st:odh_responder i) : ST (extracted_secret i)
-  (requires (fun h0 ->
-    let sr, _, n = st.key in
-    MM.fresh st.log (pubshare sr, n) h0)) // Can only call once
-  (ensures (fun h0 (sr,r) h1 ->
-    let (g, si) = ishare_of_id i in
-    let (sr, _, n) = st.key in
-    if Flags.ideal_kef then
-      DH.honestGroup g /\ DH.honest_share si ==>
-        (modifies_one st.r h0 h1 /\
-        MR.m_sel h1 st.log == MM.upd (MR.m_sel h0 st.log) (pubshare sr, n) r /\
-        witnessed (MM.contains st.log (pubshare sr, n) r))
-    else h0 = h1))
+type rshare (i:id) = (let (| g, si |) = ishare_of_id i in DH.share g)
+type rsecret (i:id) = (let (| g, si |) = ishare_of_id i in DH.secret g)
+
+// Non-terminating function to generate a fresh responder share that doesn't appear in the ODH table
+let fresh_sharegen: i:id -> log:log -> n:salt i -> ST (rshare i * rsecret i)
+  (requires (fun h0 -> True))
+  (ensures (fun h0 (sr, gxy) h1 ->
+    modifies_none h0 h1 /\
+    honest i ==> MM.fresh log (sr, n) h1))
   =
-  let g, si = ishare_of_id i in
-  let sr, secret, n = st.key in
-  if Flags.ideal_kef && DH.strongGroup g && DH.is_honest si then
-    let r = Bytes.random (keflen i.alg) in
-    m_recall st.log;
-    MM.extend st.log (pubshare sr, n) r;
-    (sr, r)
+  let sr, gxy = DH.dh_responder si in
+  if is_honest i then
+    match MM.lookup log (sr, n) with
+    | None -> (sr, gxy)
+    | Some _ -> fresh_sharegen i log n
+  else sr, gxy
+
+let prf (i:id) (gxy:extracted_secret i) (n:salt i) =
+  if DH_PSK? i.kef_type then
+    let st = KEF_PRF.create i n in // TODO memoize
+    KEF_PRF.extract i st gxy
   else
     let concrete_n = match i.kef_type with
       | DH _ _ _ -> zH (hashalg i)
       | DH_PSK _ _ _ _ -> n in
-    let r = Hacl.KEF.extract (i.alg) secret concrete_n in
+    Hacl.KEF.extract (i.alg) gxy n
+
+let extract_responder (i:id) (st:odh_responder i) : ST (rshare i * extracted_secret i)
+  (requires (fun h0 -> True))
+  (ensures (fun h0 (sr,r) h1 ->
+    let (| g, si |) = ishare_of_id i in
+    let n:salt i = st.key in
+    (if safeId i then
+      modifies_one st.r h0 h1 /\
+      MR.m_sel h1 st.log == MM.upd (MR.m_sel h0 st.log) (sr, n) r /\
+      MR.witnessed (MM.defined st.log (sr, n)) /\
+      MR.witnessed (MM.contains st.log (sr, n) r)
+    else h0 = h1)))
+  =
+  let (| g, si |) = ishare_of_id i in
+  let n : salt i = st.key in
+  let sr, gxy = fresh_sharegen i st.log n in
+  if is_honest i then
+    let r = Bytes.random (keflen i.alg) in
+    m_recall st.log;
+    MM.extend st.log (sr, n) r; // we know (sr,n) is fresh from fresh_sharegen
+    (sr, r)
+  else
+    let r = prf i gxy concrete_n in
     (sr, r)
 
-let extract_initiator (i:id) (st:odh_initiator i)
-  (sr:share (fst (ishare_of_id i)) (n:salt i)
+let extract_initiator (i:id) (st:odh_initiator i) (sr:rshare i) (n:salt i)
   : ST (extracted_secret i)
-  (requires (fun h0 -> safeId i ==> MM.defined st.log (sr, n)))
+  (requires (fun h0 ->
+    is_None (MR.m_sel st.initiator_responder h0)))
   (ensures (fun h0 r h1 ->
     let g, si = ishare_of_id i in
-    modifies_none h0 h1 /\
-    (Flags.ideal_kef /\ DH.strongGroup g /\ DH.honest_share si) ==>
-      (r == MM.value st.log (si, n))))
+    modifies_one st.r h0 h1 /\
+    safeId i /\ MR.witnessed (MM.contains st.log (sr,n)) ==>
+      (MM.defined st.log (sr,n) r h1 /\
+      HH.sel h1 st.initiator_responder == Some (sr,n))
+  ))
   =
   let g, si = ishare_of_id i in
-  let ksi = st.key in
-  let secret = DH.initiator ksi sr in
-  let concrete_n = match i.kef_type with
-    | DH _ _ _ -> zH (hashalg i)
-    | DH_PSK _ _ _ _ -> n in
-  let r = Hacl.KEF.extract (i.alg) secret concrete_n in
-  if Flags.ideal_kef && DH.strongGroup g && DH.is_honest si then
-    (match MM.lookup st.log (sr, n) with
-    | Some r -> r)
-  else r
-
-(*
-let extract (i:id) (st:state i) (ir:role i) (s:salt i)
-  : ST (odh_extracted i s)
-  (requires (fun h0 -> True))
-  (ensures (fun h0 r h1 ->
-    if Flags.ideal_kef /\ safeId i then
-      (match MM.sel (MR.m_sel h0 st.log) s with
-      | None ->
-        (ir == Initiator ==> modifies_none h0 h1) /\
-        (ir == Responder ==>
-          modifies_one st.r h0 h1 /\
-          MR.m_sel h1 st.log == MM.upd (MR.m_sel h0 st.log) s r /\
-          witnessed (MM.contains st.log s r))
-      | Some r' ->
-        modifies_none h0 h1 /\
-        r' = r)
-    else
-      h0 = h1))
-  =
-  let concrete_s =
-    match i.kef_type with
-    | DH _ _ _ -> zH (hashalg i)
-    | DH_PSK _ _ _ _ -> s in
-
-    module PRF_ODH
-
-    val strongKef: a:keflag -> GTot bool
-    val strongGroup: g:group -> GTot bool
-
-    type share (g:group)
-    val hasSecret: #g:group -> share g -> GTot bool
-    type keyshare (g:group) = s:share g{hasSecret s}
-    val honestShare: share -> GTot bool
-
-    val keysharegen: g:group -> ST (s:keyshare g)
-    val sharecoerce: g:group -> pub:bytes{length pub = elemlen g} -> ST (s:share g{~(honestShare s)})
-    val keysharecoerce: g:group -> priv:bytes{length priv = keylen g} -> ST (s:keyshare g{~(honestShare s)})
-    val pubshare: keyshare -> Tot share
-
-    type salt (k:kefalg) = b:bytes{length b = saltlen k}
-    val honestSalt: #k:kefalg -> salt k -> GTot bool
-    val psk_zero_salt: k:kefalg -> Tot (n:salt k{~(honestSalt n)})
-    val saltgen: k:kefalg -> ST (n:salt k{n <> psk_zero_salt k})
-    val saltcoerce: k:kefalg -> b:bytes{length b = saltlen k} -> ST (n:salt k{~(honestSalt n)})
-
-    type extracted_secret (k:kefalg) (g:group)
-    type safeExtract (k:kefalg) (g:group) (ks:keyshare g) (s:share g) (n:salt k) =
-      strongKef k /\ ((honestShare ks /\ honestShare s /\ strongGroup g) \/ (honestSalt n))
-
-    type dhrole =
-    | Initiator
-    | Responder
-
-    val odh_table : monotone_map (k:kefalg & g:group & s1:share g & s2:share g & n:salt k) (extracted_secret k g)
-
-    type registered_secret (k:kefalg) (g:group) (ks:keyshare g) (s:share g) (n:salt k) (h:mem) =
-      is_Some (lookup odh_table (k,g,ks,s,n) h)
-
-    type stored_secret (k:kefalg) (g:group) (ks:keyshare g) (s:share g) (n:salt k) (e:extracted_secret k g) (h:mem) =
-      registered_secret k g ks s n /\ lookup odh_table (k,g,ks,s,n) h = Some e
-
-    val extract: k:kefalg -> g:group -> role:dhrole -> ks:keyshare g -> s:share g -> n:salt k -> ST (extracted_secret k g)
-      (requires (fun h0 -> True)) // Maybe restrict to calling once per role?
-      (ensures (fun h0 r h1 ->
-        safeExtract k g ks s n ==>
-          let (s1, s2) =
-            match role with
-            | Initiator -> (pubshare ks, s)
-            | Responder -> (s, pubshare ks) in
-          match lookup odh_table (k,g,s1,s2,n) with
-          | None ->
-            m_sel h1 odh_table = update_map (m_sel h0 odh_table) (k,g,s1,s2,n) r
-          | Some r' -> r' = r
-      ))
-
-    let extract k g role ks s n =
-      if safeExtract k g ks s n then
-        let (s1, s2) =
-          match role with
-          | Initiator -> (pubshare ks, s)
-          | Responder -> (s, pubshare ks) in
-        (match m_lookup odh_table (k,g,s1,s2,n) with
-        | None ->
-           let r = KDF.gen k in
-           update_map odh_table (k,g,s1,s2,n) r; r
-        | Some r -> r)
-      else
-        let ikm = CommonDH.exponentiate g ks s in
-        HKDF.hkdf_extract k n ikm
-
-*)
+  let ksi : DH.keyshare g{DH.pubshare ksi = si} = st.key in
+  let gxy = DH.dh_initiator ksi sr in
+  if is_safe i then
+    match MM.lookup st.log (sr, n) with
+    | None -> prf i gxy n // behave concretely
+    | Some r -> st.initiator_responder := (sr, n); r
+  else
+    prf i gxy n
