src/tls/concrete-flags/Flags.fst
@@ -1,5 +1,6 @@
 module Flags
 
+inline_for_extraction let ideal_KEF = false
 inline_for_extraction let ideal_Nonce = false  
 inline_for_extraction let ideal_Sig = false
 inline_for_extraction let ideal_PMS = false
