src/tls/ideal-flags/Flags.fst
@@ -1,6 +1,7 @@
 module Flags
 
-assume val ideal_Nonce : bool  
+assume val ideal_KEF : bool
+assume val ideal_Nonce : bool 
 assume val ideal_Sig : bool 
 assume val ideal_PMS : bool 
 assume val ideal_PRF : bool 
